src/Std/Do'/Triple/SpecLemmas.lean
@@ -6,11 +6,13 @@ Authors: Vladimir Gladshtein, Sebastian Graf
 module
 
 prelude
+public import Std.Do'.Tactic.Attr
 
 public import Std.Do'.Triple.Basic
-public import Init.Data.Range.Polymorphic.Iterators
+import Init.Data.Range.Polymorphic.Iterators
 import Init.Data.Range.Polymorphic
-public import Init.Data.Slice.Array
+import Init.Data.Slice.Array
+public import Std.Do.Triple.SpecLemmas
 
 -- This public import is a workaround for #10652.
 -- Without it, adding the `spec` attribute for `instMonadLiftTOfMonadLift` will fail.
@@ -40,142 +42,142 @@ set_option linter.missingDocs true
 This module contains Hoare triple specifications for some functions in Core.
 -/
 
-namespace Std.Legacy.Range
+-- namespace Std.Legacy.Range
 
-/--
-Converts a range to the list of all numbers in the range.
--/
-abbrev toList (r : Std.Legacy.Range) : List Nat :=
-  List.range' r.start ((r.stop - r.start + r.step - 1) / r.step) r.step
+-- -- /--
+-- -- Converts a range to the list of all numbers in the range.
+-- -- -/
+-- -- abbrev toList (r : Std.Legacy.Range) : List Nat :=
+-- --   List.range' r.start ((r.stop - r.start + r.step - 1) / r.step) r.step
 
-end Std.Legacy.Range
+-- end Std.Legacy.Range
 
-namespace List
+-- namespace List
 
-/--
-A pointer at a specific location in a list. List cursors are used in loop invariants for the
-`mvcgen` tactic.
+-- /--
+-- A pointer at a specific location in a list. List cursors are used in loop invariants for the
+-- `mvcgen` tactic.
 
-Moving the cursor to the left or right takes time linear in the current position of the cursor, so
-this data structure is not appropriate for run-time code.
--/
-@[ext]
-structure Cursor {α : Type u} (l : List α) : Type u where
-  /--
-  The elements before to the current position in the list.
-  -/
-  «prefix» : List α
-  /--
-  The elements starting at the current position. If the position is after the last element of the
-  list, then the suffix is empty; otherwise, the first element of the suffix is the current element
-  that the cursor points to.
-  -/
-  suffix : List α
-  /-- Appending the prefix to the suffix yields the original list. -/
-  property : «prefix» ++ suffix = l
+-- Moving the cursor to the left or right takes time linear in the current position of the cursor, so
+-- this data structure is not appropriate for run-time code.
+-- -/
+-- @[ext]
+-- structure Cursor {α : Type u} (l : List α) : Type u where
+--   /--
+--   The elements before to the current position in the list.
+--   -/
+--   «prefix» : List α
+--   /--
+--   The elements starting at the current position. If the position is after the last element of the
+--   list, then the suffix is empty; otherwise, the first element of the suffix is the current element
+--   that the cursor points to.
+--   -/
+--   suffix : List α
+--   /-- Appending the prefix to the suffix yields the original list. -/
+--   property : «prefix» ++ suffix = l
 
-/--
-Creates a cursor at position `n` in the list `l`.
-The prefix contains the first `n` elements, and the suffix contains the remaining elements.
-If `n` is larger than the length of the list, the cursor is positioned at the end of the list.
--/
-def Cursor.at (l : List α) (n : Nat) : Cursor l := ⟨l.take n, l.drop n, by simp⟩
+-- /--
+-- Creates a cursor at position `n` in the list `l`.
+-- The prefix contains the first `n` elements, and the suffix contains the remaining elements.
+-- If `n` is larger than the length of the list, the cursor is positioned at the end of the list.
+-- -/
+-- def Cursor.at (l : List α) (n : Nat) : Cursor l := ⟨l.take n, l.drop n, by simp⟩
 
-/--
-Creates a cursor at the beginning of the list (position 0).
-The prefix is empty and the suffix is the entire list.
--/
-abbrev Cursor.begin (l : List α) : Cursor l := .at l 0
+-- /--
+-- Creates a cursor at the beginning of the list (position 0).
+-- The prefix is empty and the suffix is the entire list.
+-- -/
+-- abbrev Cursor.begin (l : List α) : Cursor l := .at l 0
 
-/--
-Creates a cursor at the end of the list.
-The prefix is the entire list and the suffix is empty.
--/
-abbrev Cursor.end (l : List α) : Cursor l := .at l l.length
+-- /--
+-- Creates a cursor at the end of the list.
+-- The prefix is the entire list and the suffix is empty.
+-- -/
+-- abbrev Cursor.end (l : List α) : Cursor l := .at l l.length
 
-/--
-Returns the element at the current cursor position.
+-- /--
+-- Returns the element at the current cursor position.
 
-Requires that is a current element: the suffix must be non-empty, so the cursor is not at the end of
-the list.
--/
-def Cursor.current {α} {l : List α} (c : Cursor l) (h : 0 < c.suffix.length := by get_elem_tactic) : α :=
-  c.suffix[0]'(by simp [h])
+-- Requires that is a current element: the suffix must be non-empty, so the cursor is not at the end of
+-- the list.
+-- -/
+-- def Cursor.current {α} {l : List α} (c : Cursor l) (h : 0 < c.suffix.length := by get_elem_tactic) : α :=
+--   c.suffix[0]'(by simp [h])
 
-/--
-Advances the cursor by one position, moving the current element from the suffix to the prefix.
+-- /--
+-- Advances the cursor by one position, moving the current element from the suffix to the prefix.
 
-Requires that the cursor is not already at the end of the list.
--/
-def Cursor.tail (s : Cursor l) (h : 0 < s.suffix.length := by get_elem_tactic) : Cursor l :=
-  { «prefix» := s.prefix ++ [s.current]
-  , suffix := s.suffix.tail
-  , property := by
-      have : s.suffix ≠ [] := by simp only [List.ne_nil_iff_length_pos, h]
-      simp [current, ←List.head_eq_getElem this, s.property] }
+-- Requires that the cursor is not already at the end of the list.
+-- -/
+-- def Cursor.tail (s : Cursor l) (h : 0 < s.suffix.length := by get_elem_tactic) : Cursor l :=
+--   { «prefix» := s.prefix ++ [s.current]
+--   , suffix := s.suffix.tail
+--   , property := by
+--       have : s.suffix ≠ [] := by simp only [List.ne_nil_iff_length_pos, h]
+--       simp [current, ←List.head_eq_getElem this, s.property] }
 
-@[simp, grind =] theorem Cursor.prefix_at (l : List α) : (Cursor.at l n).prefix = l.take n := rfl
-@[simp, grind =] theorem Cursor.suffix_at (l : List α) : (Cursor.at l n).suffix = l.drop n := rfl
-@[simp, grind =] theorem Cursor.current_at (l : List α) (h : n < l.length) :
-    (Cursor.at l n).current  (by simpa using Nat.sub_lt_sub_right (Nat.le_refl n) h) = l[n] := by
-  induction n with simp_all [Cursor.current]
-@[simp, grind =] theorem Cursor.tail_at (l : List α) (h : n < l.length) :
-    (Cursor.at l n).tail (by simpa using Nat.sub_lt_sub_right (Nat.le_refl n) h) = Cursor.at l (n + 1) := by
-  simp [Cursor.tail, Cursor.at, Cursor.current]
+-- @[simp, grind =] theorem Cursor.prefix_at (l : List α) : (Cursor.at l n).prefix = l.take n := rfl
+-- @[simp, grind =] theorem Cursor.suffix_at (l : List α) : (Cursor.at l n).suffix = l.drop n := rfl
+-- @[simp, grind =] theorem Cursor.current_at (l : List α) (h : n < l.length) :
+--     (Cursor.at l n).current  (by simpa using Nat.sub_lt_sub_right (Nat.le_refl n) h) = l[n] := by
+--   induction n with simp_all [Cursor.current]
+-- @[simp, grind =] theorem Cursor.tail_at (l : List α) (h : n < l.length) :
+--     (Cursor.at l n).tail (by simpa using Nat.sub_lt_sub_right (Nat.le_refl n) h) = Cursor.at l (n + 1) := by
+--   simp [Cursor.tail, Cursor.at, Cursor.current]
 
-/--
-The position of the cursor in the list.
-It's a shortcut for the number of elements in the prefix.
--/
-abbrev Cursor.pos (c : Cursor l) : Nat := c.prefix.length
+-- /--
+-- The position of the cursor in the list.
+-- It's a shortcut for the number of elements in the prefix.
+-- -/
+-- abbrev Cursor.pos (c : Cursor l) : Nat := c.prefix.length
 
-@[simp, grind =]
-theorem Cursor.pos_at {l : List α} {n : Nat} (h : n < l.length) :
-    (Cursor.at l n).pos = n := by simp only [pos, «at», length_take]; omega
+-- @[simp, grind =]
+-- theorem Cursor.pos_at {l : List α} {n : Nat} (h : n < l.length) :
+--     (Cursor.at l n).pos = n := by simp only [pos, «at», length_take]; omega
 
-@[simp]
-theorem Cursor.pos_mk {l pre suff : List α} (h : pre ++ suff = l) :
-    (Cursor.mk pre suff h).pos = pre.length := rfl
+-- @[simp]
+-- theorem Cursor.pos_mk {l pre suff : List α} (h : pre ++ suff = l) :
+--     (Cursor.mk pre suff h).pos = pre.length := rfl
 
-@[grind →]
-theorem eq_of_range'_eq_append_cons (h : range' s n step = xs ++ cur :: ys) :
-    cur = s + step * xs.length := by
-  rw [range'_eq_append_iff] at h
-  obtain ⟨k, hk, hxs, hcur⟩ := h
-  have h := (range'_eq_cons_iff.mp hcur.symm).1.symm
-  have hk : k = xs.length := by simp_all [length_range']
-  simp only [h, hk, Nat.add_left_cancel_iff]
-  apply Nat.mul_comm
+-- @[grind →]
+-- theorem eq_of_range'_eq_append_cons (h : range' s n step = xs ++ cur :: ys) :
+--     cur = s + step * xs.length := by
+--   rw [range'_eq_append_iff] at h
+--   obtain ⟨k, hk, hxs, hcur⟩ := h
+--   have h := (range'_eq_cons_iff.mp hcur.symm).1.symm
+--   have hk : k = xs.length := by simp_all [length_range']
+--   simp only [h, hk, Nat.add_left_cancel_iff]
+--   apply Nat.mul_comm
 
-@[grind →]
-theorem length_of_range'_eq_append_cons (h : range' s n step = xs ++ cur :: ys) :
-    n = xs.length + ys.length + 1 := by
-  have : n = (range' s n step).length := by simp
-  simpa [h] using this
+-- @[grind →]
+-- theorem length_of_range'_eq_append_cons (h : range' s n step = xs ++ cur :: ys) :
+--     n = xs.length + ys.length + 1 := by
+--   have : n = (range' s n step).length := by simp
+--   simpa [h] using this
 
-@[grind →]
-theorem mem_of_range'_eq_append_cons (h : range' s n step = xs ++ i :: ys) :
-    i ∈ range' s n step := by simp [h]
+-- @[grind →]
+-- theorem mem_of_range'_eq_append_cons (h : range' s n step = xs ++ i :: ys) :
+--     i ∈ range' s n step := by simp [h]
 
-@[grind →]
-theorem gt_of_range'_eq_append_cons (h : range' s n step = xs ++ i :: ys) (hstep : 0 < step) (hj : j ∈ xs) :
-    j < i := by
-  obtain ⟨nxs, _, rfl, htail⟩ := range'_eq_append_iff.mp h
-  obtain ⟨rfl, _⟩ := range'_eq_cons_iff.mp htail.symm
-  simp only [mem_range'] at hj
-  obtain ⟨i, _, rfl⟩ := hj
-  apply Nat.add_lt_add_left
-  simp [Nat.mul_comm, *]
+-- @[grind →]
+-- theorem gt_of_range'_eq_append_cons (h : range' s n step = xs ++ i :: ys) (hstep : 0 < step) (hj : j ∈ xs) :
+--     j < i := by
+--   obtain ⟨nxs, _, rfl, htail⟩ := range'_eq_append_iff.mp h
+--   obtain ⟨rfl, _⟩ := range'_eq_cons_iff.mp htail.symm
+--   simp only [mem_range'] at hj
+--   obtain ⟨i, _, rfl⟩ := hj
+--   apply Nat.add_lt_add_left
+--   simp [Nat.mul_comm, *]
 
-@[grind →]
-theorem lt_of_range'_eq_append_cons (h : range' s n step = xs ++ i :: ys) (hstep : 0 < step) (hj : j ∈ ys) :
-    i < j := by
-  obtain ⟨k, hk, rfl, htail⟩ := range'_eq_append_iff.mp h
-  obtain ⟨rfl, _, _, _⟩ := range'_eq_cons_iff.mp htail.symm
-  simp only [mem_range'] at hj
-  omega
+-- @[grind →]
+-- theorem lt_of_range'_eq_append_cons (h : range' s n step = xs ++ i :: ys) (hstep : 0 < step) (hj : j ∈ ys) :
+--     i < j := by
+--   obtain ⟨k, hk, rfl, htail⟩ := range'_eq_append_iff.mp h
+--   obtain ⟨rfl, _, _, _⟩ := range'_eq_cons_iff.mp htail.symm
+--   simp only [mem_range'] at hj
+--   omega
 
-end List
+-- end List
 
 
 namespace Std.Do'
@@ -187,12 +189,13 @@ variable {m : Type u → Type v} {l : Type u} {e : Type u}
 
 /-! # `Monad` -/
 
-variable [Monad m] [WPMonad m l e]
+variable [Monad m] [AssertionLang l] [ExceptAssertionLang e] [WPMonad m l e]
 
 theorem Spec.pure' (a : α) (h : pre ⊑ post a) :
     Triple pre (Pure.pure (f := m) a) post epost :=
   Triple.pure a h
 
+@[lspec]
 theorem Spec.pure (a : α) :
     Triple (post a) (Pure.pure (f := m) a) post epost :=
   Spec.pure' a PartialOrder.rel_refl
@@ -202,6 +205,7 @@ theorem Spec.bind' (x : m α) (f : α → m β)
     Triple pre (x >>= f) post epost :=
   Triple.bind x f (fun a => wp (f a) post epost) h (fun _ => Triple.iff.mpr PartialOrder.rel_refl)
 
+@[lspec]
 theorem Spec.bind (x : m α) (f : α → m β) :
     Triple (wp x (fun a => wp (f a) post epost) epost) (x >>= f) post epost :=
   Spec.bind' x f (Triple.iff.mpr PartialOrder.rel_refl)
@@ -212,6 +216,7 @@ theorem Spec.map' (f : α → β) (x : m α)
     Triple pre (f <$> x) post epost :=
   Triple.iff.mpr (PartialOrder.rel_trans (Triple.iff.mp h) (WPMonad.wp_map f x post epost))
 
+@[lspec]
 theorem Spec.map (f : α → β) (x : m α) :
     Triple (wp x (fun a => post (f a)) epost) (f <$> x) post epost :=
   Spec.map' f x (Triple.iff.mpr PartialOrder.rel_refl)
@@ -221,56 +226,54 @@ theorem Spec.seq' (x : m (α → β)) (y : m α)
     Triple pre (x <*> y) post epost :=
   Triple.iff.mpr (PartialOrder.rel_trans (Triple.iff.mp h) (WPMonad.wp_seq x y post epost))
 
+@[lspec]
 theorem Spec.seq (x : m (α → β)) (y : m α) :
     Triple (wp x (fun f => wp y (fun a => post (f a)) epost) epost) (x <*> y) post epost :=
   Spec.seq' x y (Triple.iff.mpr PartialOrder.rel_refl)
 
 /-! # `MonadLift` -/
 
+@[lspec]
 theorem Spec.monadLift_StateT (x : m α) (post : α → σ → l) :
     Triple (fun s => wp x (fun a => post a s) epost) (MonadLift.monadLift x : StateT σ m α) post epost :=
   Triple.iff.mpr (WP.monadLift_StateT_wp x post)
 
+@[lspec]
 theorem Spec.monadLift_ReaderT (x : m α) (post : α → ρ → l) :
     Triple (fun r => wp x (fun a => post a r) epost) (MonadLift.monadLift x : ReaderT ρ m α) post epost :=
   Triple.iff.mpr (by rw [WP.monadLift_ReaderT_wp]; rfl)
 
+@[lspec]
 theorem Spec.monadLift_ExceptT (x : m α) (post : α → l) (epost : EPost.cons (ε → l) e) :
     Triple (wp x post epost.tail) (MonadLift.monadLift x : ExceptT ε m α) post epost :=
   Triple.iff.mpr (WP.monadLift_ExceptT_wp x post epost)
 
 /-
+@[lspec]
 theorem Spec.monadLift_OptionT (x : m α) (post : α → l) (epost : e × l) :
     Triple (wp x post epost.1) (MonadLift.monadLift x : OptionT m α) post epost :=
   Triple.iff.mpr (monadLift_OptionT_wp x)
 -/
 
-/-! # `MonadLiftT` -/
-
-omit [Monad m] in
-theorem Spec.UnfoldLift.monadLift_trans [MonadLift n o] [MonadLiftT m n] (x : m α) :
-    (MonadLiftT.monadLift x : o α) = MonadLift.monadLift (m := n) (monadLift x) := rfl
-
-omit [Monad m] in
-theorem Spec.UnfoldLift.monadLift_refl (x : m α) :
-    (MonadLiftT.monadLift x : m α) = x := rfl
-
 /-! # `MonadFunctor` -/
 
 attribute [refl] PartialOrder.rel_refl
 
+@[lspec]
 theorem Spec.monadMap_StateT
     (f : ∀{β}, m β → m β) {α} (x : StateT σ m α) (post : α → σ → l) :
     Triple (fun s => wp (f (x.run s)) (fun (a, s') => post a s') epost)
       (MonadFunctor.monadMap (m := m) f x : StateT σ m α) post epost :=
   Triple.iff.mpr (by rw [WP.monadMap_StateT_wp]; rfl)
 
+@[lspec]
 theorem Spec.monadMap_ReaderT
     (f : ∀{β}, m β → m β) {α} (x : ReaderT ρ m α) (post : α → ρ → l) :
     Triple (fun r => wp (f (x.run r)) (fun a => post a r) epost)
       (MonadFunctor.monadMap (m := m) f x : ReaderT ρ m α) post epost :=
   Triple.iff.mpr (by rw [WP.monadMap_ReaderT_wp]; rfl)
 
+@[lspec]
 theorem Spec.monadMap_ExceptT
     (f : ∀{β}, m β → m β) {α} (x : ExceptT ε m α) (post : α → l) (epost : EPost.cons (ε → l) e) :
     Triple (wp (f x.run) (epost.pushExcept post) epost.tail)
@@ -278,6 +281,7 @@ theorem Spec.monadMap_ExceptT
   Triple.iff.mpr (by rw [WP.monadMap_ExceptT_wp])
 
 /-
+@[lspec]
 theorem Spec.monadMap_OptionT
     (f : ∀{β}, m β → m β) {α} (x : OptionT m α) (post : α → l) (epost : e × l) :
     Triple (wp (f x.run) (fun o => match o with | some a => post a | none => epost.2) epost.1)
@@ -286,6 +290,7 @@ theorem Spec.monadMap_OptionT
 -/
 
 
+@[lspec]
 theorem Spec.monadMap_refl (x : m α) :
     Triple (wp (f x : m α) post epost)
       (MonadFunctorT.monadMap f x : m α) post epost :=
@@ -293,18 +298,21 @@ theorem Spec.monadMap_refl (x : m α) :
 
 /-! # `MonadControl` -/
 
+@[lspec]
 theorem Spec.liftWith_StateT
     (f : (∀{β}, StateT σ m β → m (β × σ)) → m α) (post : α → σ → l) :
     Triple (fun s => wp (f (fun x => x.run s)) (fun a => post a s) epost)
       (MonadControl.liftWith (m:=m) f : StateT σ m α) post epost :=
   Triple.iff.mpr (by intro s; simp [WP.liftWith_StateT_wp f]; apply WPMonad.wp_map'; ext; rfl)
 
+@[lspec]
 theorem Spec.liftWith_ReaderT
     (f : (∀{β}, ReaderT ρ m β → m β) → m α) (post : α → ρ → l) :
     Triple (fun r => wp (f (fun x => x.run r)) (fun a => post a r) epost)
       (MonadControl.liftWith (m:=m) f : ReaderT ρ m α) post epost :=
   Triple.iff.mpr (by intro r; simp [WP.liftWith_ReaderT_wp f]; rfl)
 
+@[lspec]
 theorem Spec.liftWith_ExceptT
     (f : (∀{β}, ExceptT ε m β → m (Except ε β)) → m α) (post : α → l) (epost : EPost.cons (ε → l) e) :
     Triple (wp (f (fun x => x.run)) post epost.tail)
@@ -312,6 +320,7 @@ theorem Spec.liftWith_ExceptT
   Triple.iff.mpr (by simp [WP.liftWith_ExceptT_wp f]; apply WPMonad.wp_map'; ext; rfl)
 
 /-
+@[lspec]
 theorem Spec.liftWith_OptionT
     (f : (∀{β}, OptionT m β → m (Option β)) → m α) (post : α → l) (epost : e × l) :
     Triple (wp (f (fun x => x.run)) post epost.1)
@@ -319,22 +328,26 @@ theorem Spec.liftWith_OptionT
   Triple.iff.mpr (WP.liftWith_OptionT_wp f)
 -/
 
+@[lspec]
 theorem Spec.restoreM_StateT (x : m (α × σ)) (post : α → σ → l) :
     Triple (fun _ => wp x (fun (a, s) => post a s) epost)
       (MonadControl.restoreM (m:=m) x : StateT σ m α) post epost :=
   Triple.iff.mpr (WP.restoreM_StateT_wp x)
 
+@[lspec]
 theorem Spec.restoreM_ReaderT (x : m α) (post : α → ρ → l) :
     Triple (fun r => wp x (fun a => post a r) epost)
       (MonadControl.restoreM (m:=m) x : ReaderT ρ m α) post epost :=
   Triple.iff.mpr (by rw [WP.restoreM_ReaderT_wp]; rfl)
 
+@[lspec]
 theorem Spec.restoreM_ExceptT (x : m (@Except.{u, u} ε α)) (post : α → l) (epost : EPost.cons (ε → l) e) :
     Triple (wp x (epost.pushExcept post) epost.tail)
       (MonadControl.restoreM (m:=m) x : ExceptT ε m α) post epost :=
   Triple.iff.mpr (by rw [WP.restoreM_ExceptT_wp])
 
 /-
+@[lspec]
 theorem Spec.restoreM_OptionT (x : m (Option α)) (post : α → l) (epost : e × l) :
     Triple (wp x (fun (o : Option α) => match o with | some a => post a | none => epost.2) epost.1)
       (MonadControl.restoreM (m:=m) x : OptionT m α) post epost :=
@@ -344,6 +357,7 @@ theorem Spec.restoreM_OptionT (x : m (Option α)) (post : α → l) (epost : e �
 /-! # `MonadControlT` -/
 
 
+@[lspec]
 theorem Spec.liftWith_refl
     (f : (∀{β}, m β → m β) → m α) :
     Triple (wp (f (fun x => x) : m α) post epost)
@@ -351,6 +365,7 @@ theorem Spec.liftWith_refl
   Triple.iff.mpr (by rw [WP.liftWith_refl_wp])
 
 
+@[lspec]
 theorem Spec.restoreM_refl (x : stM m m α) :
     Triple (wp (Pure.pure x : m α) post epost)
       (MonadControlT.restoreM (m:=m) x : m α) post epost :=
@@ -358,16 +373,19 @@ theorem Spec.restoreM_refl (x : stM m m α) :
 
 /-! # `ReaderT` -/
 
+@[lspec]
 theorem Spec.read_ReaderT (post : ρ → ρ → l) :
     Triple (fun r => post r r)
       (MonadReaderOf.read : ReaderT ρ m ρ) post epost :=
   Triple.iff.mpr (by intro r; simpa [MonadReaderOf.read] using
     (WPMonad.wp_pure (m := m) (x := r) (post := fun a => post a r) (epost := epost)))
+@[lspec]
 theorem Spec.withReader_ReaderT (f : ρ → ρ) (x : ReaderT ρ m α) (post : α → ρ → l) :
     Triple (fun r => wp x (fun a _ => post a r) epost (f r))
       (MonadWithReaderOf.withReader f x : ReaderT ρ m α) post epost :=
   Triple.iff.mpr (by rw [WP.withReader_ReaderT_wp]; rfl)
 
+@[lspec]
 theorem Spec.adapt_ReaderT (f : ρ → ρ') (x : ReaderT ρ' m α) (post : α → ρ → l) :
     Triple (fun r => wp x (fun a _ => post a r) epost (f r))
       (ReaderT.adapt f x : ReaderT ρ m α) post epost :=
@@ -375,6 +393,7 @@ theorem Spec.adapt_ReaderT (f : ρ → ρ') (x : ReaderT ρ' m α) (post : α �
 
 /-! # `StateT` -/
 
+@[lspec]
 theorem Spec.get_StateT (post : σ → σ → l) :
     Triple (fun s => post s s)
       (MonadStateOf.get : StateT σ m σ) post epost :=
@@ -382,6 +401,7 @@ theorem Spec.get_StateT (post : σ → σ → l) :
     (WPMonad.wp_pure (m := m) (x := (s, s))
       (post := fun x => post x.fst x.snd) (epost := epost)))
 
+@[lspec]
 theorem Spec.set_StateT (s : σ) (post : PUnit → σ → l) :
     Triple (fun _ => post ⟨⟩ s)
       (set s : StateT σ m PUnit) post epost :=
@@ -389,6 +409,7 @@ theorem Spec.set_StateT (s : σ) (post : PUnit → σ → l) :
     (WPMonad.wp_pure (m := m) (x := (PUnit.unit, s))
       (post := fun x => post x.fst x.snd) (epost := epost)))
 
+@[lspec]
 theorem Spec.modifyGet_StateT (f : σ → α × σ) (post : α → σ → l) :
     Triple (fun s => post (f s).1 (f s).2)
       (MonadStateOf.modifyGet f : StateT σ m α) post epost :=
@@ -398,6 +419,7 @@ theorem Spec.modifyGet_StateT (f : σ → α × σ) (post : α → σ → l) :
 
 /-! # `ExceptT` -/
 
+@[lspec]
 theorem Spec.run_ExceptT (x : ExceptT ε m α) (post : α → l) (epost : EPost.cons (ε → l) e) :
     Triple (wp x post epost)
       (x.run : m (@Except.{u, u} ε α))
@@ -405,6 +427,7 @@ theorem Spec.run_ExceptT (x : ExceptT ε m α) (post : α → l) (epost : EPost.
       epost.tail :=
   Triple.iff.mpr (by simp [PartialOrder.rel_refl])
 
+@[lspec]
 theorem Spec.throw_ExceptT (err : ε) (post : α → l) (epost : EPost.cons (ε → l) e) :
     Triple (epost.head err) (MonadExceptOf.throw err : ExceptT ε m α) post epost :=
   Triple.iff.mpr (by simpa [EPost.cons.pushExcept] using
@@ -412,16 +435,19 @@ theorem Spec.throw_ExceptT (err : ε) (post : α → l) (epost : EPost.cons (ε 
       (post := epost.pushExcept post)
       (epost := epost.tail)))
 
+@[lspec]
 theorem Spec.tryCatch_ExceptT (x : ExceptT ε m α) (h : ε → ExceptT ε m α) (post : α → l) (epost : EPost.cons (ε → l) e) :
     Triple (wp x post ⟨fun e => wp (h e) post epost, epost.tail⟩)
       (MonadExceptOf.tryCatch x h : ExceptT ε m α) post epost :=
   Triple.iff.mpr (WP.tryCatch_ExceptT_wp x h)
 
+@[lspec]
 theorem Spec.orElse_ExceptT (x : ExceptT ε m α) (h : Unit → ExceptT ε m α) (post : α → l) (epost : EPost.cons (ε → l) e) :
     Triple (wp x post ⟨fun _ => wp (h ()) post epost, epost.tail⟩)
       (OrElse.orElse x h : ExceptT ε m α) post epost :=
   Triple.iff.mpr (WP.orElse_ExceptT_wp x h)
 
+@[lspec]
 theorem Spec.adapt_ExceptT (f : ε → ε') (x : ExceptT ε m α) (post : α → l) (epost : EPost.cons (ε' → l) e) :
     Triple (wp x post ⟨fun e => epost.head (f e), epost.tail⟩)
       (ExceptT.adapt f x : ExceptT ε' m α) post epost :=
@@ -429,15 +455,18 @@ theorem Spec.adapt_ExceptT (f : ε → ε') (x : ExceptT ε m α) (post : α →
 
 /-! # `Except` -/
 
+@[lspec]
 theorem Spec.throw_Except (err : ε) :
     Triple (epost.head err) (MonadExceptOf.throw err : Except ε α) post epost :=
   Triple.iff.mpr (by rw [WP.throw_Except_wp]; rfl)
 
+@[lspec]
 theorem Spec.tryCatch_Except (x : Except ε α) (h : ε → Except ε α) :
     Triple (wp x post epost⟨fun e => wp (h e) post epost⟩)
       (MonadExceptOf.tryCatch x h : Except ε α) post epost :=
   Triple.iff.mpr (by rw [WP.tryCatch_Except_wp]; rfl)
 
+@[lspec]
 theorem Spec.orElse_Except (x : Except ε α) (h : Unit → Except ε α) :
     Triple (wp x post epost⟨fun (_ : ε) => wp (h ()) post epost⟩)
       (OrElse.orElse x h : Except ε α) post epost :=
@@ -446,6 +475,7 @@ theorem Spec.orElse_Except (x : Except ε α) (h : Unit → Except ε α) :
 /-! # `OptionT` -/
 
 /-
+@[lspec]
 theorem Spec.run_OptionT (x : OptionT m α) (post : α → l) (epost : e × l) :
     Triple (wp x post epost)
       (x.run : m (Option α))
@@ -453,15 +483,18 @@ theorem Spec.run_OptionT (x : OptionT m α) (post : α → l) (epost : e × l) :
       epost.1 :=
   Triple.iff.mpr (by rw [← OptionT_run_wp]; rfl)
 
+@[lspec]
 theorem Spec.throw_OptionT (err : PUnit) (post : α → l) (epost : e × l) :
     Triple epost.2 (MonadExceptOf.throw err : OptionT m α) post epost :=
   Triple.iff.mpr (by rw [throw_OptionT_wp])
 
+@[lspec]
 theorem Spec.tryCatch_OptionT (x : OptionT m α) (h : PUnit → OptionT m α) (post : α → l) (epost : e × l) :
     Triple (wp x post (epost.1, wp (h ⟨⟩) post epost))
       (MonadExceptOf.tryCatch x h : OptionT m α) post epost :=
   Triple.iff.mpr (tryCatch_OptionT_wp x h)
 
+@[lspec]
 theorem Spec.orElse_OptionT (x : OptionT m α) (h : Unit → OptionT m α) (post : α → l) (epost : e × l) :
     Triple (wp x post (epost.1, wp (h ()) post epost))
       (OrElse.orElse x h : OptionT m α) post epost :=
@@ -469,15 +502,18 @@ theorem Spec.orElse_OptionT (x : OptionT m α) (h : Unit → OptionT m α) (post
 
 /-! # `Option` -/
 
+@[lspec]
 theorem Spec.throw_Option (err : PUnit) :
     Triple epost (MonadExceptOf.throw err : Option α) post epost :=
   Triple.iff.mpr (by rw [throw_Option_wp]; rfl)
 
+@[lspec]
 theorem Spec.tryCatch_Option (x : Option α) (h : PUnit → Option α) :
     Triple (wp x post (wp (h ⟨⟩) post epost))
       (MonadExceptOf.tryCatch x h : Option α) post epost :=
   Triple.iff.mpr (by rw [tryCatch_Option_wp]; rfl)
 
+@[lspec]
 theorem Spec.orElse_Option (x : Option α) (h : Unit → Option α) (post : α → Prop) (epost : Prop) :
     Triple (wp x post (wp (h ()) post epost))
       (OrElse.orElse x h : Option α) post epost :=
@@ -486,91 +522,79 @@ theorem Spec.orElse_Option (x : Option α) (h : Unit → Option α) (post : α �
 
 /-! # `EStateM` -/
 
+@[lspec]
 theorem Spec.get_EStateM (post : σ → σ → Prop) (epost : ε → σ → Prop) :
     Triple (fun s => post s s)
       (MonadStateOf.get : EStateM ε σ σ) post epost :=
   Triple.iff.mpr (by rw [WP.get_EStateM_wp]; rfl)
 
+@[lspec]
 theorem Spec.set_EStateM (s : σ) (post : PUnit → σ → Prop) (epost : ε → σ → Prop) :
     Triple (fun _ => post ⟨⟩ s)
       (MonadStateOf.set s : EStateM ε σ PUnit) post epost :=
   Triple.iff.mpr (by rw [WP.set_EStateM_wp]; rfl)
 
+@[lspec]
 theorem Spec.modifyGet_EStateM (f : σ → α × σ) (post : α → σ → Prop) (epost : ε → σ → Prop) :
     Triple (fun s => post (f s).1 (f s).2)
       (MonadStateOf.modifyGet f : EStateM ε σ α) post epost :=
   Triple.iff.mpr (by rw [WP.modifyGet_EStateM_wp]; rfl)
 
+@[lspec]
 theorem Spec.throw_EStateM (err : ε) (post : α → σ → Prop) (epost : ε → σ → Prop) :
     Triple (epost err) (MonadExceptOf.throw err : EStateM ε σ α) post epost :=
   Triple.iff.mpr (by rw [WP.throw_EStateM_wp]; rfl)
 
+@[lspec]
 theorem Spec.tryCatch_EStateM (x : EStateM ε σ α) (h : ε → EStateM ε σ α)
     (post : α → σ → Prop) (epost : ε → σ → Prop) :
     Triple (fun s => wp x post (fun e s' => wp (h e) post epost s') s)
       (MonadExceptOf.tryCatch x h : EStateM ε σ α) post epost :=
   Triple.iff.mpr (by rw [WP.tryCatch_EStateM_wp]; rfl)
 
+@[lspec]
 theorem Spec.orElse_EStateM (x : EStateM ε σ α) (h : Unit → EStateM ε σ α)
     (post : α → σ → Prop) (epost : ε → σ → Prop) :
     Triple (fun s => wp x post (fun _ s' => wp (h ()) post epost s') s)
       (OrElse.orElse x h : EStateM ε σ α) post epost :=
   Triple.iff.mpr (by rw [WP.orElse_EStateM_wp]; rfl)
 
+@[lspec]
 theorem Spec.adaptExcept_EStateM (f : ε → ε') (x : EStateM ε σ α)
     (post : α → σ → Prop) (epost : ε' → σ → Prop) :
     Triple (wp x post (fun e => epost (f e)))
       (EStateM.adaptExcept f x : EStateM ε' σ α) post epost :=
   Triple.iff.mpr (by rw [WP.adaptExcept_EStateM_wp]; rfl)
 
-/-! # Lifting `MonadStateOf` -/
-
-omit [Monad m] [WPMonad m l e] in
-theorem Spec.UnfoldLift.get [MonadLift m n] [MonadStateOf σ m] :
-    (MonadStateOf.get : n σ) = monadLift (MonadStateOf.get : m σ) := rfl
-
-omit [Monad m] [WPMonad m l e] in
-theorem Spec.UnfoldLift.set [MonadLift m n] [MonadStateOf σ m] (s : σ) :
-    (MonadStateOf.set (m := n) s) = monadLift (MonadStateOf.set (m := m) s) := rfl
-
-omit [Monad m] [WPMonad m l e] in
-theorem Spec.UnfoldLift.modifyGet [MonadLift m n] [MonadStateOf σ m] (f : σ → α × σ) :
-    MonadStateOf.modifyGet (m := n) f = monadLift (MonadStateOf.modifyGet (m := m) f) := rfl
-
-/-! # Lifting `MonadReaderOf` -/
-
-omit [Monad m] [WPMonad m l e] in
-theorem Spec.UnfoldLift.read [MonadLift m n] [MonadReaderOf ρ m] :
-    (MonadReaderOf.read : n ρ) = monadLift (MonadReaderOf.read : m ρ) := rfl
-
-omit [Monad m] [WPMonad m l e] in
-theorem Spec.UnfoldLift.withReader [MonadFunctor m n] [MonadWithReaderOf ρ m] (f : ρ → ρ) :
-    (MonadWithReaderOf.withReader f : n α → n α) = monadMap (m := m) (MonadWithReaderOf.withReader f) := rfl
-
 /-! # Lifting `MonadExceptOf` -/
 
 
+@[lspec]
 theorem Spec.throw_MonadExcept [MonadExceptOf ε m] (err : ε) :
     Triple (wp (MonadExceptOf.throw err : m α) post epost)
       (throw err : m α) post epost :=
   Triple.iff.mpr (by simp [throw, PartialOrder.rel_refl])
 
 
+@[lspec]
 theorem Spec.tryCatch_MonadExcept [MonadExceptOf ε m] (x : m α) (h : ε → m α) :
     Triple (wp (MonadExceptOf.tryCatch x h : m α) post epost)
       (tryCatch x h : m α) post epost :=
   Triple.iff.mpr (by rw [WP.tryCatch_MonadExcept_wp])
 
+@[lspec]
 theorem Spec.throw_ReaderT [MonadExceptOf ε m] (err : ε) (post : α → ρ → l) :
     Triple (wp (MonadLift.monadLift (MonadExceptOf.throw (ε:=ε) err : m α) : ReaderT ρ m α) post epost)
       (MonadExceptOf.throw (ε:=ε) err : ReaderT ρ m α) post epost :=
   Triple.iff.mpr (by rw [WP.throw_ReaderT_lift_wp]; rfl)
 
+@[lspec]
 theorem Spec.throw_StateT [MonadExceptOf ε m] (err : ε) (post : α → σ → l) :
     Triple (wp (MonadLift.monadLift (MonadExceptOf.throw (ε:=ε) err : m α) : StateT σ m α) post epost)
       (MonadExceptOf.throw (ε:=ε) err : StateT σ m α) post epost :=
   Triple.iff.mpr (by rw [WP.throw_StateT_lift_wp]; rfl)
 
+@[lspec]
 theorem Spec.throw_ExceptT_lift [MonadExceptOf ε m] (err : ε) (post : α → l) (epost : EPost.cons (ε' → l) e) :
     Triple (wp (MonadExceptOf.throw (ε:=ε) err : m (@Except.{u, u} ε' α))
         (fun r => match r with | .ok a => post a | .error e => epost.head e) epost.tail)
@@ -578,6 +602,7 @@ theorem Spec.throw_ExceptT_lift [MonadExceptOf ε m] (err : ε) (post : α → l
   Triple.iff.mpr (by rw [WP.throw_lift_ExceptT_wp]; apply WPMonad.wp_cons; intro r; cases r <;> rfl)
 
 /-
+@[lspec]
 theorem Spec.throw_Option_lift [MonadExceptOf ε m] (err : ε) (post : α → l) (epost : l × e) :
     Triple (wp (MonadExceptOf.throw (ε:=ε) err : m (Option α))
         (fun | some a => post a | none => epost.2) epost.1)
@@ -585,6 +610,7 @@ theorem Spec.throw_Option_lift [MonadExceptOf ε m] (err : ε) (post : α → l)
   Triple.iff.mpr (by rw [throw_lift_OptionT_wp]; apply WPMonad.wp_cons; intro r; cases r <;> rfl)
 -/
 
+@[lspec]
 theorem Spec.tryCatch_ReaderT [MonadExceptOf ε m] (x : ReaderT ρ m α) (h : ε → ReaderT ρ m α)
     (post : α → ρ → l) :
     Triple (fun r => wp (MonadExceptOf.tryCatch (ε:=ε) (x.run r) (fun e => (h e).run r) : m α)
@@ -592,6 +618,7 @@ theorem Spec.tryCatch_ReaderT [MonadExceptOf ε m] (x : ReaderT ρ m α) (h : ε
       (MonadExceptOf.tryCatch (ε:=ε) x h : ReaderT ρ m α) post epost :=
   Triple.iff.mpr (by rw [WP.tryCatch_ReaderT_lift_wp]; rfl)
 
+@[lspec]
 theorem Spec.tryCatch_StateT [MonadExceptOf ε m] (x : StateT σ m α) (h : ε → StateT σ m α)
     (post : α → σ → l) :
     Triple (fun s => wp (MonadExceptOf.tryCatch (ε:=ε) (x.run s) (fun e => (h e).run s) : m (α × σ))
@@ -599,6 +626,7 @@ theorem Spec.tryCatch_StateT [MonadExceptOf ε m] (x : StateT σ m α) (h : ε �
       (MonadExceptOf.tryCatch (ε:=ε) x h : StateT σ m α) post epost :=
   Triple.iff.mpr (by rw [WP.tryCatch_StateT_lift_wp]; rfl)
 
+@[lspec]
 theorem Spec.tryCatch_ExceptT_lift [MonadExceptOf ε m] (x : ExceptT ε' m α) (h : ε → ExceptT ε' m α)
     (post : α → l) (epost : EPost.cons (ε' → l) e) :
     Triple (wp (MonadExceptOf.tryCatch (ε:=ε) x h : m (@Except.{u, u} ε' α))
@@ -607,7 +635,7 @@ theorem Spec.tryCatch_ExceptT_lift [MonadExceptOf ε m] (x : ExceptT ε' m α) (
   Triple.iff.mpr (by rw [WP.tryCatch_lift_ExceptT_wp]; apply WPMonad.wp_cons; intro r; cases r <;> rfl)
 
 -- /-
---
+-- @[lspec]
 -- theorem Spec.tryCatch_OptionT_lift [MonadExceptOf ε m] (x : OptionT m α) (h : ε → OptionT m α)
 --     (post : α → l) (epost : e × l) :
 --     Triple (wp (MonadExceptOf.tryCatch (ε:=ε) x h : m (Option α))
@@ -619,6 +647,7 @@ theorem Spec.tryCatch_ExceptT_lift [MonadExceptOf ε m] (x : ExceptT ε' m α) (
 -- /-! # `MonadFunctorT` / `MonadControlT` transitivity -/
 
 
+@[lspec]
 theorem Spec.monadMap_trans
     {n₁ : Type u → Type v} {n₂ : Type u → Type v}
     [MonadFunctor n₁ m] [MonadFunctorT n₂ n₁]
@@ -629,6 +658,7 @@ theorem Spec.monadMap_trans
   Triple.iff.mpr (by rw [WP.monadMap_trans_wp])
 
 
+@[lspec]
 theorem Spec.liftWith_trans
     {n₁ : Type u → Type v} {n₂ : Type u → Type v}
     [MonadControl n₁ m] [MonadControlT n₂ n₁]
@@ -638,6 +668,7 @@ theorem Spec.liftWith_trans
   Triple.iff.mpr (by rw [WP.liftWith_trans_wp])
 
 
+@[lspec]
 theorem Spec.restoreM_trans
     {n₁ : Type u → Type v} {n₂ : Type u → Type v}
     [MonadControl n₁ m] [MonadControlT n₂ n₁]
@@ -655,7 +686,7 @@ namespace Std.Do'
 universe u₁ u₂ v
 
 variable {α : Type u₁} {β : Type (max u₁ u₂)} {m : Type (max u₁ u₂) → Type v} {l : Type (max u₁ u₂)} {e : Type (max u₁ u₂)}
-variable [Monad m] [WPMonad m l e]
+variable [Monad m] [AssertionLang l] [ExceptAssertionLang e] [WPMonad m l e]
 
 /--
 The type of loop invariants used by the specifications of `for ... in ...` loops.
@@ -670,6 +701,7 @@ abbrev Invariant {α : Type u₁} (xs : List α) (β : Type u₂)
 set_option linter.missingDocs false in
 abbrev eInvariant (e : Type u) := e
 
+@[lspec]
 theorem Spec.forIn'_list
     {xs : List α} {init : β} {f : (a : α) → a ∈ xs → β → m (ForInStep β)}
     (inv : Invariant xs β l)
@@ -712,6 +744,7 @@ theorem Spec.forIn'_list
       next => -- .done case
         apply Triple.pure; rfl
 
+@[lspec]
 theorem Spec.forIn'_list_const_inv
     {xs : List α} {init : β} {f : (a : α) → a ∈ xs → β → m (ForInStep β)}
     {inv : (β → l)}
@@ -727,6 +760,7 @@ theorem Spec.forIn'_list_const_inv
     (fun _p c _s h b => step c (by rw [h]; exact List.mem_append_right _ (List.Mem.head _)) b)
 
 
+@[lspec]
 theorem Spec.forIn_list
     {xs : List α} {init : β} {f : α → β → m (ForInStep β)}
     (inv : Invariant xs β l)
@@ -748,6 +782,7 @@ theorem Spec.forIn_list
   exact Spec.forIn'_list inv eInv step
 
 
+@[lspec]
 theorem Spec.forIn_list_const_inv
     {xs : List α} {init : β} {f : α → β → m (ForInStep β)}
     {inv : (β → l)}
@@ -761,6 +796,7 @@ theorem Spec.forIn_list_const_inv
     Triple (inv init) (forIn xs init f) inv eInv :=
   Spec.forIn_list (fun p => inv p.2) eInv (fun _p c _s _h b => step c b)
 
+@[lspec]
 theorem Spec.foldlM_list [LawfulMonad m]
     {xs : List α} {init : β} {f : β → α → m β}
     (inv : Invariant xs β l)
@@ -784,6 +820,7 @@ theorem Spec.foldlM_list [LawfulMonad m]
   apply Spec.map'
   apply step <;> assumption
 
+@[lspec]
 theorem Spec.foldlM_list_const_inv [LawfulMonad m]
     {xs : List α} {init : β} {f : β → α → m β}
     {inv : (β → l)}
@@ -797,8 +834,9 @@ theorem Spec.foldlM_list_const_inv [LawfulMonad m]
     Triple (inv init) (List.foldlM f init xs) inv eInv :=
     Spec.foldlM_list (fun p => inv p.2) eInv (fun _p c _s _h b => step c b)
 
+@[lspec]
 theorem Spec.forIn'_range {β : Type u} {m : Type u → Type v} {l : Type u} {e : Type u}
-    [Monad m] [WPMonad m l e]
+    [Monad m] [AssertionLang l] [ExceptAssertionLang e] [WPMonad m l e]
     {xs : Std.Legacy.Range} {init : β} {f : (a : Nat) → a ∈ xs → β → m (ForInStep β)}
     (inv : Invariant xs.toList β l)
     (eInv : e)
@@ -818,8 +856,9 @@ theorem Spec.forIn'_range {β : Type u} {m : Type u → Type v} {l : Type u} {e 
   simp only [Std.Legacy.Range.forIn'_eq_forIn'_range', Std.Legacy.Range.size, Std.Legacy.Range.size.eq_1]
   exact Spec.forIn'_list inv eInv (fun c hcur b => step c hcur b)
 
+@[lspec]
 theorem Spec.forIn_range {β : Type u} {m : Type u → Type v} {l : Type u} {e : Type u}
-    [Monad m] [WPMonad m l e]
+    [Monad m] [AssertionLang l] [ExceptAssertionLang e] [WPMonad m l e]
     {xs : Std.Legacy.Range} {init : β} {f : Nat → β → m (ForInStep β)}
     (inv : Invariant xs.toList β l)
     (eInv : e)
@@ -840,8 +879,9 @@ theorem Spec.forIn_range {β : Type u} {m : Type u → Type v} {l : Type u} {e :
   exact Spec.forIn_list inv eInv step
 
 open Std Std.PRange in
+@[lspec]
 theorem Spec.forIn'_rcc {α β : Type u} {m : Type u → Type v} {l : Type u} {e : Type u}
-    [Monad m] [WPMonad m l e] [LawfulMonad m]
+    [Monad m] [AssertionLang l] [ExceptAssertionLang e] [WPMonad m l e] [LawfulMonad m]
     [LE α] [DecidableLE α] [UpwardEnumerable α] [Rxc.IsAlwaysFinite α]
     [LawfulUpwardEnumerable α] [LawfulUpwardEnumerableLE α]
     {xs : Rcc α} {init : β} {f : (a : α) → a ∈ xs → β → m (ForInStep β)}
@@ -864,8 +904,9 @@ theorem Spec.forIn'_rcc {α β : Type u} {m : Type u → Type v} {l : Type u} {e
   exact Spec.forIn'_list inv eInv step
 
 open Std Std.PRange in
+@[lspec]
 theorem Spec.forIn_rcc {α β : Type u} {m : Type u → Type v} {l : Type u} {e : Type u}
-    [Monad m] [WPMonad m l e] [LawfulMonad m]
+    [Monad m] [AssertionLang l] [ExceptAssertionLang e] [WPMonad m l e] [LawfulMonad m]
     [LE α] [DecidableLE α] [UpwardEnumerable α] [Rxc.IsAlwaysFinite α]
     [LawfulUpwardEnumerable α] [LawfulUpwardEnumerableLE α]
     {xs : Rcc α} {init : β} {f : α → β → m (ForInStep β)}
@@ -888,8 +929,9 @@ theorem Spec.forIn_rcc {α β : Type u} {m : Type u → Type v} {l : Type u} {e 
   exact Spec.forIn'_rcc inv eInv step
 
 open Std Std.PRange in
+@[lspec]
 theorem Spec.forIn'_rco {α β : Type u} {m : Type u → Type v} {l : Type u} {e : Type u}
-    [Monad m] [WPMonad m l e] [LawfulMonad m]
+    [Monad m] [AssertionLang l] [ExceptAssertionLang e] [WPMonad m l e] [LawfulMonad m]
     [LE α] [LT α] [DecidableLT α] [UpwardEnumerable α] [Rxo.IsAlwaysFinite α]
     [LawfulUpwardEnumerable α] [LawfulUpwardEnumerableLE α] [LawfulUpwardEnumerableLT α]
     {xs : Rco α} {init : β} {f : (a : α) → a ∈ xs → β → m (ForInStep β)}
@@ -912,8 +954,9 @@ theorem Spec.forIn'_rco {α β : Type u} {m : Type u → Type v} {l : Type u} {e
   exact Spec.forIn'_list inv eInv step
 
 open Std Std.PRange in
+@[lspec]
 theorem Spec.forIn_rco {α β : Type u} {m : Type u → Type v} {l : Type u} {e : Type u}
-    [Monad m] [WPMonad m l e] [LawfulMonad m]
+    [Monad m] [AssertionLang l] [ExceptAssertionLang e] [WPMonad m l e] [LawfulMonad m]
     [LE α] [LT α] [DecidableLT α] [UpwardEnumerable α] [Rxo.IsAlwaysFinite α]
     [LawfulUpwardEnumerable α] [LawfulUpwardEnumerableLE α] [LawfulUpwardEnumerableLT α]
     {xs : Rco α} {init : β} {f : α → β → m (ForInStep β)}
@@ -936,8 +979,9 @@ theorem Spec.forIn_rco {α β : Type u} {m : Type u → Type v} {l : Type u} {e 
   exact Spec.forIn'_rco inv eInv step
 
 open Std Std.PRange in
+@[lspec]
 theorem Spec.forIn'_rci {α β : Type u} {m : Type u → Type v} {l : Type u} {e : Type u}
-    [Monad m] [WPMonad m l e] [LawfulMonad m]
+    [Monad m] [AssertionLang l] [ExceptAssertionLang e] [WPMonad m l e] [LawfulMonad m]
     [LE α] [UpwardEnumerable α] [Rxi.IsAlwaysFinite α]
     [LawfulUpwardEnumerable α] [LawfulUpwardEnumerableLE α]
     {xs : Rci α} {init : β} {f : (a : α) → a ∈ xs → β → m (ForInStep β)}
@@ -960,8 +1004,9 @@ theorem Spec.forIn'_rci {α β : Type u} {m : Type u → Type v} {l : Type u} {e
   exact Spec.forIn'_list inv eInv step
 
 open Std Std.PRange in
+@[lspec]
 theorem Spec.forIn_rci {α β : Type u} {m : Type u → Type v} {l : Type u} {e : Type u}
-    [Monad m] [WPMonad m l e] [LawfulMonad m]
+    [Monad m] [AssertionLang l] [ExceptAssertionLang e] [WPMonad m l e] [LawfulMonad m]
     [LE α] [UpwardEnumerable α] [Rxi.IsAlwaysFinite α]
     [LawfulUpwardEnumerable α] [LawfulUpwardEnumerableLE α]
     {xs : Rci α} {init : β} {f : α → β → m (ForInStep β)}
@@ -984,8 +1029,9 @@ theorem Spec.forIn_rci {α β : Type u} {m : Type u → Type v} {l : Type u} {e 
   exact Spec.forIn'_rci inv eInv step
 
 open Std Std.PRange in
+@[lspec]
 theorem Spec.forIn'_roc {α β : Type u} {m : Type u → Type v} {l : Type u} {e : Type u}
-    [Monad m] [WPMonad m l e] [LawfulMonad m]
+    [Monad m] [AssertionLang l] [ExceptAssertionLang e] [WPMonad m l e] [LawfulMonad m]
     [LE α] [DecidableLE α] [LT α] [UpwardEnumerable α] [Rxc.IsAlwaysFinite α]
     [LawfulUpwardEnumerable α] [LawfulUpwardEnumerableLE α] [LawfulUpwardEnumerableLT α]
     {xs : Roc α} {init : β} {f : (a : α) → a ∈ xs → β → m (ForInStep β)}
@@ -1008,8 +1054,9 @@ theorem Spec.forIn'_roc {α β : Type u} {m : Type u → Type v} {l : Type u} {e
   exact Spec.forIn'_list inv eInv step
 
 open Std Std.PRange in
+@[lspec]
 theorem Spec.forIn_roc {α β : Type u} {m : Type u → Type v} {l : Type u} {e : Type u}
-    [Monad m] [WPMonad m l e] [LawfulMonad m]
+    [Monad m] [AssertionLang l] [ExceptAssertionLang e] [WPMonad m l e] [LawfulMonad m]
     [LE α] [DecidableLE α] [LT α] [UpwardEnumerable α] [Rxc.IsAlwaysFinite α]
     [LawfulUpwardEnumerable α] [LawfulUpwardEnumerableLE α] [LawfulUpwardEnumerableLT α]
     {xs : Roc α} {init : β} {f : α → β → m (ForInStep β)}
@@ -1032,8 +1079,9 @@ theorem Spec.forIn_roc {α β : Type u} {m : Type u → Type v} {l : Type u} {e 
   exact Spec.forIn'_roc inv eInv step
 
 open Std Std.PRange in
+@[lspec]
 theorem Spec.forIn'_roo {α β : Type u} {m : Type u → Type v} {l : Type u} {e : Type u}
-    [Monad m] [WPMonad m l e] [LawfulMonad m]
+    [Monad m] [AssertionLang l] [ExceptAssertionLang e] [WPMonad m l e] [LawfulMonad m]
     [LT α] [DecidableLT α] [UpwardEnumerable α] [Rxo.IsAlwaysFinite α]
     [LawfulUpwardEnumerable α] [LawfulUpwardEnumerableLT α]
     {xs : Roo α} {init : β} {f : (a : α) → a ∈ xs → β → m (ForInStep β)}
@@ -1056,8 +1104,9 @@ theorem Spec.forIn'_roo {α β : Type u} {m : Type u → Type v} {l : Type u} {e
   exact Spec.forIn'_list inv eInv step
 
 open Std Std.PRange in
+@[lspec]
 theorem Spec.forIn_roo {α β : Type u} {m : Type u → Type v} {l : Type u} {e : Type u}
-    [Monad m] [WPMonad m l e] [LawfulMonad m]
+    [Monad m] [AssertionLang l] [ExceptAssertionLang e] [WPMonad m l e] [LawfulMonad m]
     [LT α] [DecidableLT α] [UpwardEnumerable α] [Rxo.IsAlwaysFinite α]
     [LawfulUpwardEnumerable α] [LawfulUpwardEnumerableLT α]
     {xs : Roo α} {init : β} {f : α → β → m (ForInStep β)}
@@ -1080,8 +1129,9 @@ theorem Spec.forIn_roo {α β : Type u} {m : Type u → Type v} {l : Type u} {e 
   exact Spec.forIn'_roo inv eInv step
 
 open Std Std.PRange in
+@[lspec]
 theorem Spec.forIn'_roi {α β : Type u} {m : Type u → Type v} {l : Type u} {e : Type u}
-    [Monad m] [WPMonad m l e] [LawfulMonad m]
+    [Monad m] [AssertionLang l] [ExceptAssertionLang e] [WPMonad m l e] [LawfulMonad m]
     [LT α] [DecidableLT α] [UpwardEnumerable α] [Rxi.IsAlwaysFinite α]
     [LawfulUpwardEnumerable α] [LawfulUpwardEnumerableLT α]
     {xs : Roi α} {init : β} {f : (a : α) → a ∈ xs → β → m (ForInStep β)}
@@ -1104,8 +1154,9 @@ theorem Spec.forIn'_roi {α β : Type u} {m : Type u → Type v} {l : Type u} {e
   exact Spec.forIn'_list inv eInv step
 
 open Std Std.PRange in
+@[lspec]
 theorem Spec.forIn_roi {α β : Type u} {m : Type u → Type v} {l : Type u} {e : Type u}
-    [Monad m] [WPMonad m l e] [LawfulMonad m]
+    [Monad m] [AssertionLang l] [ExceptAssertionLang e] [WPMonad m l e] [LawfulMonad m]
     [LT α] [DecidableLT α] [UpwardEnumerable α] [Rxi.IsAlwaysFinite α]
     [LawfulUpwardEnumerable α] [LawfulUpwardEnumerableLT α]
     {xs : Roi α} {init : β} {f : α → β → m (ForInStep β)}
@@ -1128,8 +1179,9 @@ theorem Spec.forIn_roi {α β : Type u} {m : Type u → Type v} {l : Type u} {e 
   exact Spec.forIn'_roi inv eInv step
 
 open Std Std.PRange in
+@[lspec]
 theorem Spec.forIn'_ric {α β : Type u} {m : Type u → Type v} {l : Type u} {e : Type u}
-    [Monad m] [WPMonad m l e] [LawfulMonad m]
+    [Monad m] [AssertionLang l] [ExceptAssertionLang e] [WPMonad m l e] [LawfulMonad m]
     [Least? α] [LE α] [DecidableLE α] [UpwardEnumerable α] [Rxc.IsAlwaysFinite α]
     [LawfulUpwardEnumerable α] [LawfulUpwardEnumerableLeast? α] [LawfulUpwardEnumerableLE α]
     {xs : Ric α} {init : β} {f : (a : α) → a ∈ xs → β → m (ForInStep β)}
@@ -1152,8 +1204,9 @@ theorem Spec.forIn'_ric {α β : Type u} {m : Type u → Type v} {l : Type u} {e
   exact Spec.forIn'_list inv eInv step
 
 open Std Std.PRange in
+@[lspec]
 theorem Spec.forIn_ric {α β : Type u} {m : Type u → Type v} {l : Type u} {e : Type u}
-    [Monad m] [WPMonad m l e] [LawfulMonad m]
+    [Monad m] [AssertionLang l] [ExceptAssertionLang e] [WPMonad m l e] [LawfulMonad m]
     [Least? α] [LE α] [DecidableLE α] [UpwardEnumerable α] [Rxc.IsAlwaysFinite α]
     [LawfulUpwardEnumerable α] [LawfulUpwardEnumerableLeast? α] [LawfulUpwardEnumerableLE α]
     {xs : Ric α} {init : β} {f : α → β → m (ForInStep β)}
@@ -1176,8 +1229,9 @@ theorem Spec.forIn_ric {α β : Type u} {m : Type u → Type v} {l : Type u} {e 
   exact Spec.forIn'_ric inv eInv step
 
 open Std Std.PRange in
+@[lspec]
 theorem Spec.forIn'_rio {α β : Type u} {m : Type u → Type v} {l : Type u} {e : Type u}
-    [Monad m] [WPMonad m l e] [LawfulMonad m]
+    [Monad m] [AssertionLang l] [ExceptAssertionLang e] [WPMonad m l e] [LawfulMonad m]
     [Least? α] [LT α] [DecidableLT α] [UpwardEnumerable α] [Rxo.IsAlwaysFinite α]
     [LawfulUpwardEnumerable α] [LawfulUpwardEnumerableLeast? α] [LawfulUpwardEnumerableLT α]
     {xs : Rio α} {init : β} {f : (a : α) → a ∈ xs → β → m (ForInStep β)}
@@ -1200,8 +1254,9 @@ theorem Spec.forIn'_rio {α β : Type u} {m : Type u → Type v} {l : Type u} {e
   exact Spec.forIn'_list inv eInv step
 
 open Std Std.PRange in
+@[lspec]
 theorem Spec.forIn_rio {α β : Type u} {m : Type u → Type v} {l : Type u} {e : Type u}
-    [Monad m] [WPMonad m l e] [LawfulMonad m]
+    [Monad m] [AssertionLang l] [ExceptAssertionLang e] [WPMonad m l e] [LawfulMonad m]
     [Least? α] [LT α] [DecidableLT α] [UpwardEnumerable α] [Rxo.IsAlwaysFinite α]
     [LawfulUpwardEnumerable α] [LawfulUpwardEnumerableLeast? α] [LawfulUpwardEnumerableLT α]
     {xs : Rio α} {init : β} {f : α → β → m (ForInStep β)}
@@ -1224,8 +1279,9 @@ theorem Spec.forIn_rio {α β : Type u} {m : Type u → Type v} {l : Type u} {e 
   exact Spec.forIn'_rio inv eInv step
 
 open Std Std.PRange in
+@[lspec]
 theorem Spec.forIn'_rii {α β : Type u} {m : Type u → Type v} {l : Type u} {e : Type u}
-    [Monad m] [WPMonad m l e] [LawfulMonad m]
+    [Monad m] [AssertionLang l] [ExceptAssertionLang e] [WPMonad m l e] [LawfulMonad m]
     [Least? α] [UpwardEnumerable α] [Rxi.IsAlwaysFinite α]
     [LawfulUpwardEnumerable α] [LawfulUpwardEnumerableLeast? α]
     {xs : Rii α} {init : β} {f : (a : α) → a ∈ xs → β → m (ForInStep β)}
@@ -1248,8 +1304,9 @@ theorem Spec.forIn'_rii {α β : Type u} {m : Type u → Type v} {l : Type u} {e
   exact Spec.forIn'_list inv eInv step
 
 open Std Std.PRange in
+@[lspec]
 theorem Spec.forIn_rii {α β : Type u} {m : Type u → Type v} {l : Type u} {e : Type u}
-    [Monad m] [WPMonad m l e] [LawfulMonad m]
+    [Monad m] [AssertionLang l] [ExceptAssertionLang e] [WPMonad m l e] [LawfulMonad m]
     [Least? α] [UpwardEnumerable α] [Rxi.IsAlwaysFinite α]
     [LawfulUpwardEnumerable α] [LawfulUpwardEnumerableLeast? α]
     {xs : Rii α} {init : β} {f : α → β → m (ForInStep β)}
@@ -1272,8 +1329,9 @@ theorem Spec.forIn_rii {α β : Type u} {m : Type u → Type v} {l : Type u} {e 
   exact Spec.forIn'_rii inv eInv step
 
 open Std Std.Iterators in
+@[lspec]
 theorem Spec.forIn_slice {δ : Type u} {m : Type u → Type w} {l : Type u} {e : Type u}
-    [Monad m] [WPMonad m l e] [LawfulMonad m]
+    [Monad m] [AssertionLang l] [ExceptAssertionLang e] [WPMonad m l e] [LawfulMonad m]
     {γ : Type u'} {α β : Type u}
     [ToIterator (Slice γ) Id α β]
     [Iterator α Id β]
@@ -1300,8 +1358,9 @@ theorem Spec.forIn_slice {δ : Type u} {m : Type u → Type w} {l : Type u} {e :
 section Iterators
 open Std Std.Iterators
 
+@[lspec]
 theorem Spec.forIn_iter {α β γ : Type u} {m : Type u → Type w} {l : Type u} {e : Type u}
-    [Monad m] [WPMonad m l e] [LawfulMonad m]
+    [Monad m] [AssertionLang l] [ExceptAssertionLang e] [WPMonad m l e] [LawfulMonad m]
     [Iterator α Id β] [Finite α Id] [IteratorLoop α Id m] [LawfulIteratorLoop α Id m]
     {init : γ} {f : β → γ → m (ForInStep γ)}
     {it : Iter (α := α) β}
@@ -1320,8 +1379,9 @@ theorem Spec.forIn_iter {α β γ : Type u} {m : Type u → Type w} {l : Type u}
   simp only [← Iter.forIn_toList]
   exact Spec.forIn_list inv eInv step
 
+@[lspec]
 theorem Spec.forIn_iterM_id {α β γ : Type u} {m : Type u → Type w} {l : Type u} {e : Type u}
-    [Monad m] [WPMonad m l e] [LawfulMonad m]
+    [Monad m] [AssertionLang l] [ExceptAssertionLang e] [WPMonad m l e] [LawfulMonad m]
     [Iterator α Id β] [Finite α Id] [IteratorLoop α Id m] [LawfulIteratorLoop α Id m]
     {init : γ} {f : β → γ → m (ForInStep γ)}
     {it : IterM (α := α) Id β}
@@ -1342,8 +1402,9 @@ theorem Spec.forIn_iterM_id {α β γ : Type u} {m : Type u → Type w} {l : Typ
       IterM.toList_toIter]
   exact Spec.forIn_list inv eInv step
 
+@[lspec]
 theorem Spec.foldM_iter {α β γ : Type u} {m : Type u → Type w} {l : Type u} {e : Type u}
-    [Monad m] [WPMonad m l e] [LawfulMonad m]
+    [Monad m] [AssertionLang l] [ExceptAssertionLang e] [WPMonad m l e] [LawfulMonad m]
     [Iterator α Id β] [Finite α Id] [IteratorLoop α Id m] [LawfulIteratorLoop α Id m]
     {it : Iter (α := α) β}
     {init : γ} {f : γ → β → m γ}
@@ -1360,8 +1421,9 @@ theorem Spec.foldM_iter {α β γ : Type u} {m : Type u → Type w} {l : Type u}
   rw [← Iter.foldlM_toList]
   exact Spec.foldlM_list inv eInv step
 
+@[lspec]
 theorem Spec.foldM_iterM_id {α β γ : Type u} {m : Type u → Type w} {l : Type u} {e : Type u}
-    [Monad m] [WPMonad m l e] [LawfulMonad m]
+    [Monad m] [AssertionLang l] [ExceptAssertionLang e] [WPMonad m l e] [LawfulMonad m]
     [Iterator α Id β] [Finite α Id] [IteratorLoop α Id m] [LawfulIteratorLoop α Id m]
     {it : IterM (α := α) Id β}
     {init : γ} {f : γ → β → m γ}
@@ -1378,10 +1440,11 @@ theorem Spec.foldM_iterM_id {α β γ : Type u} {m : Type u → Type w} {l : Typ
   rw [← IterM.foldlM_toList]
   exact Spec.foldlM_list inv eInv step
 
+@[lspec]
 theorem Spec.IterM.forIn_filterMapWithPostcondition {α β β₂ γ : Type w}
     {m : Type w → Type w'} {n : Type w → Type w''} {o : Type w → Type w'''}
     {l : Type w} {e : Type w}
-    [Monad m] [LawfulMonad m] [Monad n] [LawfulMonad n] [Monad o] [LawfulMonad o] [WPMonad o l e]
+    [Monad m] [LawfulMonad m] [Monad n] [LawfulMonad n] [Monad o] [LawfulMonad o] [AssertionLang l] [ExceptAssertionLang e] [WPMonad o l e]
     [MonadLiftT m n] [LawfulMonadLiftT m n] [MonadLiftT n o] [LawfulMonadLiftT n o]
     [Iterator α m β] [Finite α m]
     [IteratorLoop α m o] [LawfulIteratorLoop α m o]
@@ -1396,10 +1459,11 @@ theorem Spec.IterM.forIn_filterMapWithPostcondition {α β β₂ γ : Type w}
     Triple P (forIn (it.filterMapWithPostcondition f) init g) Q eQ := by
   rwa [Std.IterM.forIn_filterMapWithPostcondition]
 
+@[lspec]
 theorem Spec.IterM.forIn_filterMapM {α β β₂ γ : Type w}
     {m : Type w → Type w'} {n : Type w → Type w''} {o : Type w → Type w'''}
     {l : Type w} {e : Type w}
-    [Monad m] [LawfulMonad m] [Monad n] [LawfulMonad n] [Monad o] [LawfulMonad o] [WPMonad o l e]
+    [Monad m] [LawfulMonad m] [Monad n] [LawfulMonad n] [Monad o] [LawfulMonad o] [AssertionLang l] [ExceptAssertionLang e] [WPMonad o l e]
     [MonadAttach n] [WeaklyLawfulMonadAttach n]
     [MonadLiftT m n] [LawfulMonadLiftT m n] [MonadLiftT n o] [LawfulMonadLiftT n o]
     [Iterator α m β] [Finite α m]
@@ -1415,10 +1479,11 @@ theorem Spec.IterM.forIn_filterMapM {α β β₂ γ : Type w}
     Triple P (forIn (it.filterMapM f) init g) Q eQ := by
   rwa [Std.IterM.forIn_filterMapM]
 
+@[lspec]
 theorem Spec.IterM.forIn_filterMap {α β β₂ γ : Type w}
     {m : Type w → Type w'} {n : Type w → Type w''}
     {l : Type w} {e : Type w}
-    [Monad m] [LawfulMonad m] [Monad n] [LawfulMonad n] [WPMonad n l e]
+    [Monad m] [LawfulMonad m] [Monad n] [LawfulMonad n] [AssertionLang l] [ExceptAssertionLang e] [WPMonad n l e]
     [MonadLiftT m n] [LawfulMonadLiftT m n]
     [Iterator α m β] [Finite α m]
     [IteratorLoop α m n] [LawfulIteratorLoop α m n]
@@ -1431,10 +1496,11 @@ theorem Spec.IterM.forIn_filterMap {α β β₂ γ : Type w}
     Triple P (forIn (it.filterMap f) init g) Q eQ := by
   rwa [Std.IterM.forIn_filterMap]
 
+@[lspec]
 theorem Spec.IterM.forIn_mapWithPostcondition {α β β₂ γ : Type w}
     {m : Type w → Type w'} {n : Type w → Type w''} {o : Type w → Type w'''}
     {l : Type w} {e : Type w}
-    [Monad m] [LawfulMonad m] [Monad n] [LawfulMonad n] [Monad o] [LawfulMonad o] [WPMonad o l e]
+    [Monad m] [LawfulMonad m] [Monad n] [LawfulMonad n] [Monad o] [LawfulMonad o] [AssertionLang l] [ExceptAssertionLang e] [WPMonad o l e]
     [MonadLiftT m n] [LawfulMonadLiftT m n] [MonadLiftT n o] [LawfulMonadLiftT n o]
     [Iterator α m β] [Finite α m]
     [IteratorLoop α m o] [LawfulIteratorLoop α m o]
@@ -1446,10 +1512,11 @@ theorem Spec.IterM.forIn_mapWithPostcondition {α β β₂ γ : Type w}
     Triple P (forIn (it.mapWithPostcondition f) init g) Q eQ := by
   rwa [Std.IterM.forIn_mapWithPostcondition]
 
+@[lspec]
 theorem Spec.IterM.forIn_mapM {α β β₂ γ : Type w}
     {m : Type w → Type w'} {n : Type w → Type w''} {o : Type w → Type w'''}
     {l : Type w} {e : Type w}
-    [Monad m] [LawfulMonad m] [Monad n] [LawfulMonad n] [Monad o] [LawfulMonad o] [WPMonad o l e]
+    [Monad m] [LawfulMonad m] [Monad n] [LawfulMonad n] [Monad o] [LawfulMonad o] [AssertionLang l] [ExceptAssertionLang e] [WPMonad o l e]
     [MonadAttach n] [WeaklyLawfulMonadAttach n]
     [MonadLiftT m n] [LawfulMonadLiftT m n] [MonadLiftT n o] [LawfulMonadLiftT n o]
     [Iterator α m β] [Finite α m]
@@ -1462,10 +1529,11 @@ theorem Spec.IterM.forIn_mapM {α β β₂ γ : Type w}
     Triple P (forIn (it.mapM f) init g) Q eQ := by
   rwa [Std.IterM.forIn_mapM]
 
+@[lspec]
 theorem Spec.IterM.forIn_map {α β β₂ γ : Type w}
     {m : Type w → Type w'} {n : Type w → Type w''}
     {l : Type w} {e : Type w}
-    [Monad m] [LawfulMonad m] [Monad n] [LawfulMonad n] [WPMonad n l e]
+    [Monad m] [LawfulMonad m] [Monad n] [LawfulMonad n] [AssertionLang l] [ExceptAssertionLang e] [WPMonad n l e]
     [MonadLiftT m n] [LawfulMonadLiftT m n]
     [Iterator α m β] [Finite α m] [IteratorLoop α m n] [LawfulIteratorLoop α m n]
     {it : IterM (α := α) m β} {f : β → β₂} {init : γ} {g : β₂ → γ → n (ForInStep γ)}
@@ -1474,10 +1542,11 @@ theorem Spec.IterM.forIn_map {α β β₂ γ : Type w}
     Triple P (forIn (it.map f) init g) Q eQ := by
   rwa [Std.IterM.forIn_map]
 
+@[lspec]
 theorem Spec.IterM.forIn_filterWithPostcondition {α β γ : Type w}
     {m : Type w → Type w'} {n : Type w → Type w''} {o : Type w → Type w'''}
     {l : Type w} {e : Type w}
-    [Monad m] [LawfulMonad m] [Monad n] [LawfulMonad n] [Monad o] [LawfulMonad o] [WPMonad o l e]
+    [Monad m] [LawfulMonad m] [Monad n] [LawfulMonad n] [Monad o] [LawfulMonad o] [AssertionLang l] [ExceptAssertionLang e] [WPMonad o l e]
     [MonadLiftT m n] [LawfulMonadLiftT m n] [MonadLiftT n o] [LawfulMonadLiftT n o]
     [Iterator α m β] [Finite α m]
     [IteratorLoop α m o] [LawfulIteratorLoop α m o]
@@ -1489,10 +1558,11 @@ theorem Spec.IterM.forIn_filterWithPostcondition {α β γ : Type w}
     Triple P (forIn (it.filterWithPostcondition f) init g) Q eQ := by
   rwa [Std.IterM.forIn_filterWithPostcondition]
 
+@[lspec]
 theorem Spec.IterM.forIn_filterM {α β γ : Type w}
     {m : Type w → Type w'} {n : Type w → Type w''} {o : Type w → Type w'''}
     {l : Type w} {e : Type w}
-    [Monad m] [LawfulMonad m] [Monad n] [LawfulMonad n] [Monad o] [LawfulMonad o] [WPMonad o l e]
+    [Monad m] [LawfulMonad m] [Monad n] [LawfulMonad n] [Monad o] [LawfulMonad o] [AssertionLang l] [ExceptAssertionLang e] [WPMonad o l e]
     [MonadAttach n] [WeaklyLawfulMonadAttach n]
     [MonadLiftT m n] [LawfulMonadLiftT m n] [MonadLiftT n o] [LawfulMonadLiftT n o]
     [Iterator α m β] [Finite α m]
@@ -1505,10 +1575,11 @@ theorem Spec.IterM.forIn_filterM {α β γ : Type w}
     Triple P (forIn (it.filterM f) init g) Q eQ := by
   rwa [Std.IterM.forIn_filterM]
 
+@[lspec]
 theorem Spec.IterM.forIn_filter {α β γ : Type w}
     {m : Type w → Type w'} {n : Type w → Type w''}
     {l : Type w} {e : Type w}
-    [Monad m] [LawfulMonad m] [Monad n] [LawfulMonad n] [WPMonad n l e]
+    [Monad m] [LawfulMonad m] [Monad n] [LawfulMonad n] [AssertionLang l] [ExceptAssertionLang e] [WPMonad n l e]
     [MonadLiftT m n] [LawfulMonadLiftT m n]
     [Iterator α m β] [Finite α m] [IteratorLoop α m n] [LawfulIteratorLoop α m n]
     {it : IterM (α := α) m β} {f : β → Bool} {init : γ} {g : β → γ → n (ForInStep γ)}
@@ -1517,11 +1588,12 @@ theorem Spec.IterM.forIn_filter {α β γ : Type w}
     Triple P (forIn (it.filter f) init g) Q eQ := by
   rwa [Std.IterM.forIn_filter]
 
+@[lspec]
 theorem Spec.IterM.foldM_filterMapWithPostcondition {α β γ δ : Type w}
     {m : Type w → Type w'} {n : Type w → Type w''} {o : Type w → Type w'''}
     {l : Type w} {e : Type w}
     [Iterator α m β] [Finite α m]
-    [Monad m] [Monad n] [Monad o] [LawfulMonad m] [LawfulMonad n] [LawfulMonad o] [WPMonad o l e]
+    [Monad m] [Monad n] [Monad o] [LawfulMonad m] [LawfulMonad n] [LawfulMonad o] [AssertionLang l] [ExceptAssertionLang e] [WPMonad o l e]
     [IteratorLoop α m n] [IteratorLoop α m o]
     [LawfulIteratorLoop α m n] [LawfulIteratorLoop α m o]
     [MonadLiftT m n] [MonadLiftT n o] [LawfulMonadLiftT m n] [LawfulMonadLiftT n o]
@@ -1535,13 +1607,14 @@ theorem Spec.IterM.foldM_filterMapWithPostcondition {α β γ δ : Type w}
     Triple P ((it.filterMapWithPostcondition f).foldM (init := init) g) Q eQ := by
   rwa [Std.IterM.foldM_filterMapWithPostcondition]
 
+@[lspec]
 theorem Spec.IterM.foldM_filterMapM {α β γ δ : Type w}
     {m : Type w → Type w'} {n : Type w → Type w''} {o : Type w → Type w'''}
     {l : Type w} {e : Type w}
     [Iterator α m β] [Finite α m]
     [Monad m] [LawfulMonad m]
     [Monad n] [MonadAttach n] [LawfulMonad n] [WeaklyLawfulMonadAttach n]
-    [Monad o] [LawfulMonad o] [WPMonad o l e]
+    [Monad o] [LawfulMonad o] [AssertionLang l] [ExceptAssertionLang e] [WPMonad o l e]
     [IteratorLoop α m n] [IteratorLoop α m o]
     [LawfulIteratorLoop α m n] [LawfulIteratorLoop α m o]
     [MonadLiftT m n] [MonadLiftT n o] [LawfulMonadLiftT m n] [LawfulMonadLiftT n o]
@@ -1555,11 +1628,12 @@ theorem Spec.IterM.foldM_filterMapM {α β γ δ : Type w}
     Triple P ((it.filterMapM f).foldM (init := init) g) Q eQ := by
   rwa [Std.IterM.foldM_filterMapM]
 
+@[lspec]
 theorem Spec.IterM.foldM_mapWithPostcondition {α β γ δ : Type w}
     {m : Type w → Type w'} {n : Type w → Type w''} {o : Type w → Type w'''}
     {l : Type w} {e : Type w}
     [Iterator α m β] [Finite α m]
-    [Monad m] [Monad n] [Monad o] [LawfulMonad m] [LawfulMonad n] [LawfulMonad o] [WPMonad o l e]
+    [Monad m] [Monad n] [Monad o] [LawfulMonad m] [LawfulMonad n] [LawfulMonad o] [AssertionLang l] [ExceptAssertionLang e] [WPMonad o l e]
     [IteratorLoop α m n] [IteratorLoop α m o]
     [LawfulIteratorLoop α m n] [LawfulIteratorLoop α m o]
     [MonadLiftT m n] [MonadLiftT n o] [LawfulMonadLiftT m n] [LawfulMonadLiftT n o]
@@ -1571,13 +1645,14 @@ theorem Spec.IterM.foldM_mapWithPostcondition {α β γ δ : Type w}
     Triple P ((it.mapWithPostcondition f).foldM (init := init) g) Q eQ := by
   rwa [Std.IterM.foldM_mapWithPostcondition]
 
+@[lspec]
 theorem Spec.IterM.foldM_mapM {α β γ δ : Type w}
     {m : Type w → Type w'} {n : Type w → Type w''} {o : Type w → Type w'''}
     {l : Type w} {e : Type w}
     [Iterator α m β] [Finite α m]
     [Monad m] [LawfulMonad m]
     [Monad n] [MonadAttach n] [LawfulMonad n] [WeaklyLawfulMonadAttach n]
-    [Monad o] [LawfulMonad o] [WPMonad o l e]
+    [Monad o] [LawfulMonad o] [AssertionLang l] [ExceptAssertionLang e] [WPMonad o l e]
     [IteratorLoop α m n] [IteratorLoop α m o]
     [LawfulIteratorLoop α m n] [LawfulIteratorLoop α m o]
     [MonadLiftT m n] [MonadLiftT n o] [LawfulMonadLiftT m n] [LawfulMonadLiftT n o]
@@ -1589,11 +1664,12 @@ theorem Spec.IterM.foldM_mapM {α β γ δ : Type w}
     Triple P ((it.mapM f).foldM (init := init) g) Q eQ := by
   rwa [Std.IterM.foldM_mapM]
 
+@[lspec]
 theorem Spec.IterM.foldM_filterWithPostcondition {α β δ : Type w}
     {m : Type w → Type w'} {n : Type w → Type w''} {o : Type w → Type w'''}
     {l : Type w} {e : Type w}
     [Iterator α m β] [Finite α m]
-    [Monad m] [Monad n] [Monad o] [LawfulMonad m] [LawfulMonad n] [LawfulMonad o] [WPMonad o l e]
+    [Monad m] [Monad n] [Monad o] [LawfulMonad m] [LawfulMonad n] [LawfulMonad o] [AssertionLang l] [ExceptAssertionLang e] [WPMonad o l e]
     [IteratorLoop α m n] [IteratorLoop α m o]
     [LawfulIteratorLoop α m n] [LawfulIteratorLoop α m o]
     [MonadLiftT m n] [MonadLiftT n o] [LawfulMonadLiftT m n] [LawfulMonadLiftT n o]
@@ -1605,13 +1681,14 @@ theorem Spec.IterM.foldM_filterWithPostcondition {α β δ : Type w}
     Triple P ((it.filterWithPostcondition f).foldM (init := init) g) Q eQ := by
   rwa [Std.IterM.foldM_filterWithPostcondition]
 
+@[lspec]
 theorem Spec.IterM.foldM_filterM {α β δ : Type w}
     {m : Type w → Type w'} {n : Type w → Type w''} {o : Type w → Type w'''}
     {l : Type w} {e : Type w}
     [Iterator α m β] [Finite α m]
     [Monad m] [LawfulMonad m]
     [Monad n] [MonadAttach n] [LawfulMonad n] [WeaklyLawfulMonadAttach n]
-    [Monad o] [LawfulMonad o] [WPMonad o l e]
+    [Monad o] [LawfulMonad o] [AssertionLang l] [ExceptAssertionLang e] [WPMonad o l e]
     [IteratorLoop α m n] [IteratorLoop α m o]
     [LawfulIteratorLoop α m n] [LawfulIteratorLoop α m o]
     [MonadLiftT m n] [MonadLiftT n o] [LawfulMonadLiftT m n] [LawfulMonadLiftT n o]
@@ -1623,10 +1700,11 @@ theorem Spec.IterM.foldM_filterM {α β δ : Type w}
     Triple P ((it.filterM f).foldM (init := init) g) Q eQ := by
   rwa [Std.IterM.foldM_filterM]
 
+@[lspec]
 theorem Spec.IterM.foldM_filterMap {α β γ δ : Type w}
     {m : Type w → Type w'} {n : Type w → Type w''}
     {l : Type w} {e : Type w}
-    [Iterator α m β] [Finite α m] [Monad m] [Monad n] [LawfulMonad m] [LawfulMonad n] [WPMonad n l e]
+    [Iterator α m β] [Finite α m] [Monad m] [Monad n] [LawfulMonad m] [LawfulMonad n] [AssertionLang l] [ExceptAssertionLang e] [WPMonad n l e]
     [IteratorLoop α m n]
     [LawfulIteratorLoop α m n]
     [MonadLiftT m n] [LawfulMonadLiftT m n]
@@ -1638,10 +1716,11 @@ theorem Spec.IterM.foldM_filterMap {α β γ δ : Type w}
     Triple P ((it.filterMap f).foldM (init := init) g) Q eQ := by
   rwa [Std.IterM.foldM_filterMap]
 
+@[lspec]
 theorem Spec.IterM.foldM_map {α β γ δ : Type w}
     {m : Type w → Type w'} {n : Type w → Type w''}
     {l : Type w} {e : Type w}
-    [Iterator α m β] [Finite α m] [Monad m] [Monad n] [LawfulMonad m] [LawfulMonad n] [WPMonad n l e]
+    [Iterator α m β] [Finite α m] [Monad m] [Monad n] [LawfulMonad m] [LawfulMonad n] [AssertionLang l] [ExceptAssertionLang e] [WPMonad n l e]
     [IteratorLoop α m n] [LawfulIteratorLoop α m n]
     [MonadLiftT m n] [LawfulMonadLiftT m n]
     {f : β → γ} {g : δ → γ → n δ} {init : δ} {it : IterM (α := α) m β}
@@ -1650,10 +1729,11 @@ theorem Spec.IterM.foldM_map {α β γ δ : Type w}
     Triple P ((it.map f).foldM (init := init) g) Q eQ := by
   rwa [Std.IterM.foldM_map]
 
+@[lspec]
 theorem Spec.IterM.foldM_filter {α β δ : Type w}
     {m : Type w → Type w'} {n : Type w → Type w''}
     {l : Type w} {e : Type w}
-    [Iterator α m β] [Finite α m] [Monad m] [Monad n] [LawfulMonad m] [LawfulMonad n] [WPMonad n l e]
+    [Iterator α m β] [Finite α m] [Monad m] [Monad n] [LawfulMonad m] [LawfulMonad n] [AssertionLang l] [ExceptAssertionLang e] [WPMonad n l e]
     [IteratorLoop α m n]
     [LawfulIteratorLoop α m n]
     [MonadLiftT m n] [LawfulMonadLiftT m n]
@@ -1663,12 +1743,13 @@ theorem Spec.IterM.foldM_filter {α β δ : Type w}
     Triple P ((it.filter f).foldM (init := init) g) Q eQ := by
   rwa [Std.IterM.foldM_filter]
 
+@[lspec]
 theorem Spec.IterM.fold_filterMapWithPostcondition {α β γ δ : Type w}
     {m : Type w → Type w'} {n : Type w → Type w''}
     {l : Type w} {e : Type w}
     [Iterator α m β] [Finite α m]
     [Monad m] [LawfulMonad m]
-    [Monad n] [LawfulMonad n] [WPMonad n l e]
+    [Monad n] [LawfulMonad n] [AssertionLang l] [ExceptAssertionLang e] [WPMonad n l e]
     [IteratorLoop α m n] [LawfulIteratorLoop α m n]
     [MonadLiftT m n] [LawfulMonadLiftT m n]
     {f : β → PostconditionT n (Option γ)} {g : δ → γ → δ} {init : δ} {it : IterM (α := α) m β}
@@ -1679,12 +1760,13 @@ theorem Spec.IterM.fold_filterMapWithPostcondition {α β γ δ : Type w}
     Triple P ((it.filterMapWithPostcondition f).fold (init := init) g) Q eQ := by
   rwa [Std.IterM.fold_filterMapWithPostcondition]
 
+@[lspec]
 theorem Spec.IterM.fold_filterMapM {α β γ δ : Type w}
     {m : Type w → Type w'} {n : Type w → Type w''}
     {l : Type w} {e : Type w}
     [Iterator α m β] [Finite α m]
     [Monad m] [LawfulMonad m]
-    [Monad n] [MonadAttach n] [LawfulMonad n] [WeaklyLawfulMonadAttach n] [WPMonad n l e]
+    [Monad n] [MonadAttach n] [LawfulMonad n] [WeaklyLawfulMonadAttach n] [AssertionLang l] [ExceptAssertionLang e] [WPMonad n l e]
     [IteratorLoop α m n] [LawfulIteratorLoop α m n]
     [MonadLiftT m n] [LawfulMonadLiftT m n]
     {f : β → n (Option γ)} {g : δ → γ → δ} {init : δ} {it : IterM (α := α) m β}
@@ -1695,12 +1777,13 @@ theorem Spec.IterM.fold_filterMapM {α β γ δ : Type w}
     Triple P ((it.filterMapM f).fold (init := init) g) Q eQ := by
   rwa [Std.IterM.fold_filterMapM]
 
+@[lspec]
 theorem Spec.IterM.fold_mapWithPostcondition {α β γ δ : Type w}
     {m : Type w → Type w'} {n : Type w → Type w''}
     {l : Type w} {e : Type w}
     [Iterator α m β] [Finite α m]
     [Monad m] [LawfulMonad m]
-    [Monad n] [LawfulMonad n] [WPMonad n l e]
+    [Monad n] [LawfulMonad n] [AssertionLang l] [ExceptAssertionLang e] [WPMonad n l e]
     [IteratorLoop α m n] [LawfulIteratorLoop α m n]
     [MonadLiftT m n] [LawfulMonadLiftT m n]
     {f : β → PostconditionT n γ} {g : δ → γ → δ} {init : δ} {it : IterM (α := α) m β}
@@ -1709,12 +1792,13 @@ theorem Spec.IterM.fold_mapWithPostcondition {α β γ δ : Type w}
     Triple P ((it.mapWithPostcondition f).fold (init := init) g) Q eQ := by
   rwa [Std.IterM.fold_mapWithPostcondition]
 
+@[lspec]
 theorem Spec.IterM.fold_mapM {α β γ δ : Type w}
     {m : Type w → Type w'} {n : Type w → Type w''}
     {l : Type w} {e : Type w}
     [Iterator α m β] [Finite α m]
     [Monad m] [LawfulMonad m]
-    [Monad n] [MonadAttach n] [LawfulMonad n] [WeaklyLawfulMonadAttach n] [WPMonad n l e]
+    [Monad n] [MonadAttach n] [LawfulMonad n] [WeaklyLawfulMonadAttach n] [AssertionLang l] [ExceptAssertionLang e] [WPMonad n l e]
     [IteratorLoop α m n] [LawfulIteratorLoop α m n]
     [MonadLiftT m n] [LawfulMonadLiftT m n]
     {f : β → n γ} {g : δ → γ → δ} {init : δ} {it : IterM (α := α) m β}
@@ -1723,12 +1807,13 @@ theorem Spec.IterM.fold_mapM {α β γ δ : Type w}
     Triple P ((it.mapM f).fold (init := init) g) Q eQ := by
   rwa [Std.IterM.fold_mapM]
 
+@[lspec]
 theorem Spec.IterM.fold_filterWithPostcondition {α β δ : Type w}
     {m : Type w → Type w'} {n : Type w → Type w''}
     {l : Type w} {e : Type w}
     [Iterator α m β] [Finite α m]
     [Monad m] [LawfulMonad m]
-    [Monad n] [LawfulMonad n] [WPMonad n l e]
+    [Monad n] [LawfulMonad n] [AssertionLang l] [ExceptAssertionLang e] [WPMonad n l e]
     [IteratorLoop α m n] [LawfulIteratorLoop α m n]
     [MonadLiftT m n] [LawfulMonadLiftT m n]
     {f : β → PostconditionT n (ULift Bool)} {g : δ → β → δ} {init : δ} {it : IterM (α := α) m β}
@@ -1737,12 +1822,13 @@ theorem Spec.IterM.fold_filterWithPostcondition {α β δ : Type w}
     Triple P ((it.filterWithPostcondition f).fold (init := init) g) Q eQ := by
   rwa [Std.IterM.fold_filterWithPostcondition]
 
+@[lspec]
 theorem Spec.IterM.fold_filterM {α β δ : Type w}
     {m : Type w → Type w'} {n : Type w → Type w''}
     {l : Type w} {e : Type w}
     [Iterator α m β] [Finite α m]
     [Monad m] [LawfulMonad m]
-    [Monad n] [MonadAttach n] [LawfulMonad n] [WeaklyLawfulMonadAttach n] [WPMonad n l e]
+    [Monad n] [MonadAttach n] [LawfulMonad n] [WeaklyLawfulMonadAttach n] [AssertionLang l] [ExceptAssertionLang e] [WPMonad n l e]
     [IteratorLoop α m n] [LawfulIteratorLoop α m n]
     [MonadLiftT m n] [LawfulMonadLiftT m n]
     {f : β → n (ULift Bool)} {g : δ → β → δ} {init : δ} {it : IterM (α := α) m β}
@@ -1751,10 +1837,11 @@ theorem Spec.IterM.fold_filterM {α β δ : Type w}
     Triple P ((it.filterM f).fold (init := init) g) Q eQ := by
   rwa [Std.IterM.fold_filterM]
 
+@[lspec]
 theorem Spec.IterM.fold_filterMap {α β γ δ : Type w}
     {m : Type w → Type w'}
     {l : Type w} {e : Type w}
-    [Iterator α m β] [Finite α m] [Monad m] [LawfulMonad m] [WPMonad m l e]
+    [Iterator α m β] [Finite α m] [Monad m] [LawfulMonad m] [AssertionLang l] [ExceptAssertionLang e] [WPMonad m l e]
     [IteratorLoop α m m] [LawfulIteratorLoop α m m]
     {f : β → Option γ} {g : δ → γ → δ} {init : δ} {it : IterM (α := α) m β}
     {P : l} {Q : δ → l} {eQ : e}
@@ -1765,10 +1852,11 @@ theorem Spec.IterM.fold_filterMap {α β γ δ : Type w}
     Triple P ((it.filterMap f).fold (init := init) g) Q eQ := by
   rwa [Std.IterM.fold_filterMap]
 
+@[lspec]
 theorem Spec.IterM.fold_map {α β γ δ : Type w}
     {m : Type w → Type w'}
     {l : Type w} {e : Type w}
-    [Iterator α m β] [Finite α m] [Monad m] [LawfulMonad m] [WPMonad m l e]
+    [Iterator α m β] [Finite α m] [Monad m] [LawfulMonad m] [AssertionLang l] [ExceptAssertionLang e] [WPMonad m l e]
     [IteratorLoop α m m] [LawfulIteratorLoop α m m]
     {f : β → γ} {g : δ → γ → δ} {init : δ} {it : IterM (α := α) m β}
     {P : l} {Q : δ → l} {eQ : e}
@@ -1776,10 +1864,11 @@ theorem Spec.IterM.fold_map {α β γ δ : Type w}
     Triple P ((it.map f).fold (init := init) g) Q eQ := by
   rwa [Std.IterM.fold_map]
 
+@[lspec]
 theorem Spec.IterM.fold_filter {α β δ : Type w}
     {m : Type w → Type w'}
     {l : Type w} {e : Type w}
-    [Iterator α m β] [Finite α m] [Monad m] [LawfulMonad m] [WPMonad m l e]
+    [Iterator α m β] [Finite α m] [Monad m] [LawfulMonad m] [AssertionLang l] [ExceptAssertionLang e] [WPMonad m l e]
     [IteratorLoop α m m] [LawfulIteratorLoop α m m]
     {f : β → Bool} {g : δ → β → δ} {init : δ} {it : IterM (α := α) m β}
     {P : l} {Q : δ → l} {eQ : e}
@@ -1787,11 +1876,12 @@ theorem Spec.IterM.fold_filter {α β δ : Type w}
     Triple P ((it.filter f).fold (init := init) g) Q eQ := by
   rwa [Std.IterM.fold_filter]
 
+@[lspec]
 theorem Spec.Iter.forIn_filterMapWithPostcondition {α β β₂ γ : Type w}
     {n : Type w → Type w'} {o : Type w → Type w''}
     {l : Type w} {e : Type w}
     [Iterator α Id β]
-    [Monad n] [LawfulMonad n] [Monad o] [LawfulMonad o] [WPMonad o l e]
+    [Monad n] [LawfulMonad n] [Monad o] [LawfulMonad o] [AssertionLang l] [ExceptAssertionLang e] [WPMonad o l e]
     [MonadLiftT n o] [LawfulMonadLiftT n o] [Finite α Id]
     [IteratorLoop α Id o] [LawfulIteratorLoop α Id o]
     {it : Iter (α := α) β} {f : β → PostconditionT n (Option β₂)} {init : γ}
@@ -1803,11 +1893,12 @@ theorem Spec.Iter.forIn_filterMapWithPostcondition {α β β₂ γ : Type w}
     Triple P (forIn (it.filterMapWithPostcondition f) init g) Q eQ := by
   rwa [Std.Iter.forIn_filterMapWithPostcondition]
 
+@[lspec]
 theorem Spec.Iter.forIn_filterMapM {α β β₂ γ : Type w}
     {n : Type w → Type w'} {o : Type w → Type w''}
     {l : Type w} {e : Type w}
     [Iterator α Id β]
-    [Monad n] [LawfulMonad n] [Monad o] [LawfulMonad o] [WPMonad o l e]
+    [Monad n] [LawfulMonad n] [Monad o] [LawfulMonad o] [AssertionLang l] [ExceptAssertionLang e] [WPMonad o l e]
     [MonadAttach n] [WeaklyLawfulMonadAttach n]
     [MonadLiftT n o] [LawfulMonadLiftT n o]
     [Finite α Id] [IteratorLoop α Id o] [LawfulIteratorLoop α Id o]
@@ -1820,11 +1911,12 @@ theorem Spec.Iter.forIn_filterMapM {α β β₂ γ : Type w}
     Triple P (forIn (it.filterMapM f) init g) Q eQ := by
   rwa [Std.Iter.forIn_filterMapM]
 
+@[lspec]
 theorem Spec.Iter.forIn_filterMap {α β β₂ γ : Type w}
     {n : Type w → Type w'}
     {l : Type w} {e : Type w}
     [Iterator α Id β]
-    [Monad n] [LawfulMonad n] [WPMonad n l e] [Finite α Id]
+    [Monad n] [LawfulMonad n] [AssertionLang l] [ExceptAssertionLang e] [WPMonad n l e] [Finite α Id]
     [IteratorLoop α Id n] [LawfulIteratorLoop α Id n]
     {it : Iter (α := α) β} {f : β → Option β₂} {init : γ} {g : β₂ → γ → n (ForInStep γ)}
     {P : l} {Q : γ → l} {eQ : e}
@@ -1835,11 +1927,12 @@ theorem Spec.Iter.forIn_filterMap {α β β₂ γ : Type w}
     Triple P (forIn (it.filterMap f) init g) Q eQ := by
   rwa [Std.Iter.forIn_filterMap]
 
+@[lspec]
 theorem Spec.Iter.forIn_mapWithPostcondition {α β β₂ γ : Type w}
     {n : Type w → Type w'} {o : Type w → Type w''}
     {l : Type w} {e : Type w}
     [Iterator α Id β]
-    [Monad n] [LawfulMonad n] [Monad o] [LawfulMonad o] [WPMonad o l e]
+    [Monad n] [LawfulMonad n] [Monad o] [LawfulMonad o] [AssertionLang l] [ExceptAssertionLang e] [WPMonad o l e]
     [MonadLiftT n o] [LawfulMonadLiftT n o] [Finite α Id]
     [IteratorLoop α Id o] [LawfulIteratorLoop α Id o]
     {it : Iter (α := α) β} {f : β → PostconditionT n β₂} {init : γ}
@@ -1848,11 +1941,12 @@ theorem Spec.Iter.forIn_mapWithPostcondition {α β β₂ γ : Type w}
     Triple P (forIn (it.mapWithPostcondition f) init g) Q eQ := by
   rwa [Std.Iter.forIn_mapWithPostcondition]
 
+@[lspec]
 theorem Spec.Iter.forIn_mapM {α β β₂ γ : Type w}
     {n : Type w → Type w'} {o : Type w → Type w''}
     {l : Type w} {e : Type w}
     [Iterator α Id β]
-    [Monad n] [LawfulMonad n] [Monad o] [LawfulMonad o] [WPMonad o l e]
+    [Monad n] [LawfulMonad n] [Monad o] [LawfulMonad o] [AssertionLang l] [ExceptAssertionLang e] [WPMonad o l e]
     [MonadAttach n] [WeaklyLawfulMonadAttach n]
     [MonadLiftT n o] [LawfulMonadLiftT n o]
     [Finite α Id]
@@ -1863,11 +1957,12 @@ theorem Spec.Iter.forIn_mapM {α β β₂ γ : Type w}
     Triple P (forIn (it.mapM f) init g) Q eQ := by
   rwa [Std.Iter.forIn_mapM]
 
+@[lspec]
 theorem Spec.Iter.forIn_map {α β β₂ γ : Type w}
     {n : Type w → Type w'}
     {l : Type w} {e : Type w}
     [Iterator α Id β]
-    [Monad n] [LawfulMonad n] [WPMonad n l e]
+    [Monad n] [LawfulMonad n] [AssertionLang l] [ExceptAssertionLang e] [WPMonad n l e]
     [Finite α Id] [IteratorLoop α Id n] [LawfulIteratorLoop α Id n]
     {it : Iter (α := α) β} {f : β → β₂} {init : γ} {g : β₂ → γ → n (ForInStep γ)}
     {P : l} {Q : γ → l} {eQ : e}
@@ -1875,11 +1970,12 @@ theorem Spec.Iter.forIn_map {α β β₂ γ : Type w}
     Triple P (forIn (it.map f) init g) Q eQ := by
   rwa [Std.Iter.forIn_map]
 
+@[lspec]
 theorem Spec.Iter.forIn_filterWithPostcondition {α β γ : Type w}
     {n : Type w → Type w'} {o : Type w → Type w''}
     {l : Type w} {e : Type w}
     [Iterator α Id β]
-    [Monad n] [LawfulMonad n] [Monad o] [LawfulMonad o] [WPMonad o l e]
+    [Monad n] [LawfulMonad n] [Monad o] [LawfulMonad o] [AssertionLang l] [ExceptAssertionLang e] [WPMonad o l e]
     [MonadLiftT n o] [LawfulMonadLiftT n o]
     [Finite α Id] [IteratorLoop α Id o] [LawfulIteratorLoop α Id o]
     {it : Iter (α := α) β} {f : β → PostconditionT n (ULift Bool)} {init : γ}
@@ -1888,11 +1984,12 @@ theorem Spec.Iter.forIn_filterWithPostcondition {α β γ : Type w}
     Triple P (forIn (it.filterWithPostcondition f) init g) Q eQ := by
   rwa [Std.Iter.forIn_filterWithPostcondition]
 
+@[lspec]
 theorem Spec.Iter.forIn_filterM {α β γ : Type w}
     {n : Type w → Type w'} {o : Type w → Type w''}
     {l : Type w} {e : Type w}
     [Iterator α Id β]
-    [Monad n] [LawfulMonad n] [Monad o] [LawfulMonad o] [WPMonad o l e]
+    [Monad n] [LawfulMonad n] [Monad o] [LawfulMonad o] [AssertionLang l] [ExceptAssertionLang e] [WPMonad o l e]
     [MonadAttach n] [WeaklyLawfulMonadAttach n]
     [MonadLiftT n o] [LawfulMonadLiftT n o] [Finite α Id]
     [IteratorLoop α Id o] [LawfulIteratorLoop α Id o]
@@ -1902,11 +1999,12 @@ theorem Spec.Iter.forIn_filterM {α β γ : Type w}
     Triple P (forIn (it.filterM f) init g) Q eQ := by
   rwa [Std.Iter.forIn_filterM]
 
+@[lspec]
 theorem Spec.Iter.forIn_filter {α β γ : Type w}
     {n : Type w → Type w'}
     {l : Type w} {e : Type w}
     [Iterator α Id β]
-    [Monad n] [LawfulMonad n] [WPMonad n l e]
+    [Monad n] [LawfulMonad n] [AssertionLang l] [ExceptAssertionLang e] [WPMonad n l e]
     [Finite α Id] [IteratorLoop α Id n] [LawfulIteratorLoop α Id n]
     {it : Iter (α := α) β} {f : β → Bool} {init : γ} {g : β → γ → n (ForInStep γ)}
     {P : l} {Q : γ → l} {eQ : e}
@@ -1914,11 +2012,12 @@ theorem Spec.Iter.forIn_filter {α β γ : Type w}
     Triple P (forIn (it.filter f) init g) Q eQ := by
   rwa [Std.Iter.forIn_filter]
 
-theorem Iter.foldM_filterMapWithPostcondition {α β γ δ : Type w}
+@[lspec]
+theorem Spec.Iter.foldM_filterMapWithPostcondition {α β γ δ : Type w}
     {n : Type w → Type w'} {o : Type w → Type w''}
     {l : Type w} {e : Type w}
     [Iterator α Id β] [Finite α Id]
-    [Monad n] [Monad o] [LawfulMonad n] [LawfulMonad o] [WPMonad o l e]
+    [Monad n] [Monad o] [LawfulMonad n] [LawfulMonad o] [AssertionLang l] [ExceptAssertionLang e] [WPMonad o l e]
     [IteratorLoop α Id n] [IteratorLoop α Id o]
     [LawfulIteratorLoop α Id n] [LawfulIteratorLoop α Id o]
     [MonadLiftT n o] [LawfulMonadLiftT n o]
@@ -1930,12 +2029,13 @@ theorem Iter.foldM_filterMapWithPostcondition {α β γ δ : Type w}
     Triple P ((it.filterMapWithPostcondition f).foldM (init := init) g) Q eQ := by
   rwa [Std.Iter.foldM_filterMapWithPostcondition]
 
-theorem Iter.foldM_filterMapM {α β γ δ : Type w}
+@[lspec]
+theorem Spec.Iter.foldM_filterMapM {α β γ δ : Type w}
     {n : Type w → Type w'} {o : Type w → Type w''}
     {l : Type w} {e : Type w}
     [Iterator α Id β] [Finite α Id]
     [Monad n] [MonadAttach n] [LawfulMonad n] [WeaklyLawfulMonadAttach n]
-    [Monad o] [LawfulMonad o] [WPMonad o l e]
+    [Monad o] [LawfulMonad o] [AssertionLang l] [ExceptAssertionLang e] [WPMonad o l e]
     [IteratorLoop α Id n] [IteratorLoop α Id o]
     [LawfulIteratorLoop α Id n] [LawfulIteratorLoop α Id o]
     [MonadLiftT n o] [LawfulMonadLiftT n o]
@@ -1947,11 +2047,12 @@ theorem Iter.foldM_filterMapM {α β γ δ : Type w}
     Triple P ((it.filterMapM f).foldM (init := init) g) Q eQ := by
   rwa [Std.Iter.foldM_filterMapM]
 
-theorem Iter.foldM_mapWithPostcondition {α β γ δ : Type w}
+@[lspec]
+theorem Spec.Iter.foldM_mapWithPostcondition {α β γ δ : Type w}
     {m : Type w → Type w'''} {n : Type w → Type w'} {o : Type w → Type w''}
     {l : Type w} {e : Type w}
     [Iterator α Id β] [Finite α Id]
-    [Monad m] [Monad n] [Monad o] [LawfulMonad m] [LawfulMonad n] [LawfulMonad o] [WPMonad o l e]
+    [Monad m] [Monad n] [Monad o] [LawfulMonad m] [LawfulMonad n] [LawfulMonad o] [AssertionLang l] [ExceptAssertionLang e] [WPMonad o l e]
     [IteratorLoop α Id n] [IteratorLoop α Id o]
     [LawfulIteratorLoop α Id n] [LawfulIteratorLoop α Id o]
     [MonadLiftT n o] [LawfulMonadLiftT n o]
@@ -1961,12 +2062,13 @@ theorem Iter.foldM_mapWithPostcondition {α β γ δ : Type w}
     Triple P ((it.mapWithPostcondition f).foldM (init := init) g) Q eQ := by
   rwa [Std.Iter.foldM_mapWithPostcondition (m := m)]
 
-theorem Iter.foldM_mapM {α β γ δ : Type w}
+@[lspec]
+theorem Spec.Iter.foldM_mapM {α β γ δ : Type w}
     {n : Type w → Type w'} {o : Type w → Type w''}
     {l : Type w} {e : Type w}
     [Iterator α Id β] [Finite α Id]
     [Monad n] [MonadAttach n] [LawfulMonad n] [WeaklyLawfulMonadAttach n]
-    [Monad o] [LawfulMonad o] [WPMonad o l e]
+    [Monad o] [LawfulMonad o] [AssertionLang l] [ExceptAssertionLang e] [WPMonad o l e]
     [IteratorLoop α Id n] [IteratorLoop α Id o]
     [LawfulIteratorLoop α Id n] [LawfulIteratorLoop α Id o]
     [MonadLiftT n o] [LawfulMonadLiftT n o]
@@ -1976,11 +2078,12 @@ theorem Iter.foldM_mapM {α β γ δ : Type w}
     Triple P ((it.mapM f).foldM (init := init) g) Q eQ := by
   rwa [Std.Iter.foldM_mapM]
 
-theorem Iter.foldM_filterWithPostcondition {α β δ : Type w}
+@[lspec]
+theorem Spec.Iter.foldM_filterWithPostcondition {α β δ : Type w}
     {n : Type w → Type w'} {o : Type w → Type w''}
     {l : Type w} {e : Type w}
     [Iterator α Id β] [Finite α Id]
-    [Monad n] [Monad o] [LawfulMonad n] [LawfulMonad o] [WPMonad o l e]
+    [Monad n] [Monad o] [LawfulMonad n] [LawfulMonad o] [AssertionLang l] [ExceptAssertionLang e] [WPMonad o l e]
     [IteratorLoop α Id n] [IteratorLoop α Id o]
     [LawfulIteratorLoop α Id n] [LawfulIteratorLoop α Id o]
     [MonadLiftT n o] [LawfulMonadLiftT n o]
@@ -1990,12 +2093,13 @@ theorem Iter.foldM_filterWithPostcondition {α β δ : Type w}
     Triple P ((it.filterWithPostcondition f).foldM (init := init) g) Q eQ := by
   rwa [Std.Iter.foldM_filterWithPostcondition]
 
-theorem Iter.foldM_filterM {α β δ : Type w}
+@[lspec]
+theorem Spec.Iter.foldM_filterM {α β δ : Type w}
     {n : Type w → Type w'} {o : Type w → Type w''}
     {l : Type w} {e : Type w}
     [Iterator α Id β] [Finite α Id]
     [Monad n] [MonadAttach n] [LawfulMonad n] [WeaklyLawfulMonadAttach n]
-    [Monad o] [LawfulMonad o] [WPMonad o l e]
+    [Monad o] [LawfulMonad o] [AssertionLang l] [ExceptAssertionLang e] [WPMonad o l e]
     [IteratorLoop α Id n] [IteratorLoop α Id o]
     [LawfulIteratorLoop α Id n] [LawfulIteratorLoop α Id o]
     [MonadLiftT n o] [LawfulMonadLiftT n o]
@@ -2005,10 +2109,11 @@ theorem Iter.foldM_filterM {α β δ : Type w}
     Triple P ((it.filterM f).foldM (init := init) g) Q eQ := by
   rwa [Std.Iter.foldM_filterM]
 
-theorem Iter.foldM_filterMap {α β γ δ : Type w}
+@[lspec]
+theorem Spec.Iter.foldM_filterMap {α β γ δ : Type w}
     {n : Type w → Type w'}
     {l : Type w} {e : Type w}
-    [Iterator α Id β] [Finite α Id] [Monad n] [LawfulMonad n] [WPMonad n l e]
+    [Iterator α Id β] [Finite α Id] [Monad n] [LawfulMonad n] [AssertionLang l] [ExceptAssertionLang e] [WPMonad n l e]
     [IteratorLoop α Id n]
     [LawfulIteratorLoop α Id n]
     {f : β → Option γ} {g : δ → γ → n δ} {init : δ} {it : Iter (α := α) β}
@@ -2019,10 +2124,11 @@ theorem Iter.foldM_filterMap {α β γ δ : Type w}
     Triple P ((it.filterMap f).foldM (init := init) g) Q eQ := by
   rwa [Std.Iter.foldM_filterMap]
 
-theorem Iter.foldM_map {α β γ δ : Type w}
+@[lspec]
+theorem Spec.Iter.foldM_map {α β γ δ : Type w}
     {n : Type w → Type w'}
     {l : Type w} {e : Type w}
-    [Iterator α Id β] [Finite α Id] [Monad n] [LawfulMonad n] [WPMonad n l e]
+    [Iterator α Id β] [Finite α Id] [Monad n] [LawfulMonad n] [AssertionLang l] [ExceptAssertionLang e] [WPMonad n l e]
     [IteratorLoop α Id n] [LawfulIteratorLoop α Id n]
     {f : β → γ} {g : δ → γ → n δ} {init : δ} {it : Iter (α := α) β}
     {P : l} {Q : δ → l} {eQ : e}
@@ -2030,10 +2136,11 @@ theorem Iter.foldM_map {α β γ δ : Type w}
     Triple P ((it.map f).foldM (init := init) g) Q eQ := by
   rwa [Std.Iter.foldM_map]
 
-theorem Iter.foldM_filter {α β δ : Type w}
+@[lspec]
+theorem Spec.Iter.foldM_filter {α β δ : Type w}
     {n : Type w → Type w'}
     {l : Type w} {e : Type w}
-    [Iterator α Id β] [Finite α Id] [Monad n] [LawfulMonad n] [WPMonad n l e]
+    [Iterator α Id β] [Finite α Id] [Monad n] [LawfulMonad n] [AssertionLang l] [ExceptAssertionLang e] [WPMonad n l e]
     [IteratorLoop α Id n] [LawfulIteratorLoop α Id n]
     {f : β → Bool} {g : δ → β → n δ} {init : δ} {it : Iter (α := α) β}
     {P : l} {Q : δ → l} {eQ : e}
@@ -2041,11 +2148,12 @@ theorem Iter.foldM_filter {α β δ : Type w}
     Triple P ((it.filter f).foldM (init := init) g) Q eQ := by
   rwa [Std.Iter.foldM_filter]
 
-theorem Iter.fold_filterMapWithPostcondition {α β γ δ : Type w}
+@[lspec]
+theorem Spec.Iter.fold_filterMapWithPostcondition {α β γ δ : Type w}
     {n : Type w → Type w'}
     {l : Type w} {e : Type w}
     [Iterator α Id β] [Finite α Id]
-    [Monad n] [LawfulMonad n] [WPMonad n l e]
+    [Monad n] [LawfulMonad n] [AssertionLang l] [ExceptAssertionLang e] [WPMonad n l e]
     [IteratorLoop α Id n] [LawfulIteratorLoop α Id n]
     {f : β → PostconditionT n (Option γ)} {g : δ → γ → δ} {init : δ} {it : Iter (α := α) β}
     {P : l} {Q : δ → l} {eQ : e}
@@ -2055,11 +2163,12 @@ theorem Iter.fold_filterMapWithPostcondition {α β γ δ : Type w}
     Triple P ((it.filterMapWithPostcondition f).fold (init := init) g) Q eQ := by
   rwa [Std.Iter.fold_filterMapWithPostcondition]
 
-theorem Iter.fold_filterMapM {α β γ δ : Type w}
+@[lspec]
+theorem Spec.Iter.fold_filterMapM {α β γ δ : Type w}
     {n : Type w → Type w'}
     {l : Type w} {e : Type w}
     [Iterator α Id β] [Finite α Id]
-    [Monad n] [MonadAttach n] [LawfulMonad n] [WeaklyLawfulMonadAttach n] [WPMonad n l e]
+    [Monad n] [MonadAttach n] [LawfulMonad n] [WeaklyLawfulMonadAttach n] [AssertionLang l] [ExceptAssertionLang e] [WPMonad n l e]
     [IteratorLoop α Id n] [LawfulIteratorLoop α Id n]
     {f : β → n (Option γ)} {g : δ → γ → δ} {init : δ} {it : Iter (α := α) β}
     {P : l} {Q : δ → l} {eQ : e}
@@ -2069,11 +2178,12 @@ theorem Iter.fold_filterMapM {α β γ δ : Type w}
     Triple P ((it.filterMapM f).fold (init := init) g) Q eQ := by
   rwa [Std.Iter.fold_filterMapM]
 
-theorem Iter.fold_mapWithPostcondition {α β γ δ : Type w}
+@[lspec]
+theorem Spec.Iter.fold_mapWithPostcondition {α β γ δ : Type w}
     {n : Type w → Type w'}
     {l : Type w} {e : Type w}
     [Iterator α Id β] [Finite α Id]
-    [Monad n] [LawfulMonad n] [WPMonad n l e]
+    [Monad n] [LawfulMonad n] [AssertionLang l] [ExceptAssertionLang e] [WPMonad n l e]
     [IteratorLoop α Id n] [LawfulIteratorLoop α Id n]
     {f : β → PostconditionT n γ} {g : δ → γ → δ} {init : δ} {it : Iter (α := α) β}
     {P : l} {Q : δ → l} {eQ : e}
@@ -2081,11 +2191,12 @@ theorem Iter.fold_mapWithPostcondition {α β γ δ : Type w}
     Triple P ((it.mapWithPostcondition f).fold (init := init) g) Q eQ := by
   rwa [Std.Iter.fold_mapWithPostcondition]
 
-theorem Iter.fold_mapM {α β γ δ : Type w}
+@[lspec]
+theorem Spec.Iter.fold_mapM {α β γ δ : Type w}
     {n : Type w → Type w'}
     {l : Type w} {e : Type w}
     [Iterator α Id β] [Finite α Id]
-    [Monad n] [MonadAttach n] [LawfulMonad n] [WeaklyLawfulMonadAttach n] [WPMonad n l e]
+    [Monad n] [MonadAttach n] [LawfulMonad n] [WeaklyLawfulMonadAttach n] [AssertionLang l] [ExceptAssertionLang e] [WPMonad n l e]
     [IteratorLoop α Id n] [LawfulIteratorLoop α Id n]
     {f : β → n γ} {g : δ → γ → δ} {init : δ} {it : Iter (α := α) β}
     {P : l} {Q : δ → l} {eQ : e}
@@ -2093,11 +2204,12 @@ theorem Iter.fold_mapM {α β γ δ : Type w}
     Triple P ((it.mapM f).fold (init := init) g) Q eQ := by
   rwa [Std.Iter.fold_mapM]
 
-theorem Iter.fold_filterWithPostcondition {α β δ : Type w}
+@[lspec]
+theorem Spec.Iter.fold_filterWithPostcondition {α β δ : Type w}
     {n : Type w → Type w'}
     {l : Type w} {e : Type w}
     [Iterator α Id β] [Finite α Id]
-    [Monad n] [LawfulMonad n] [WPMonad n l e]
+    [Monad n] [LawfulMonad n] [AssertionLang l] [ExceptAssertionLang e] [WPMonad n l e]
     [IteratorLoop α Id n] [LawfulIteratorLoop α Id n]
     {f : β → PostconditionT n (ULift Bool)} {g : δ → β → δ} {init : δ} {it : Iter (α := α) β}
     {P : l} {Q : δ → l} {eQ : e}
@@ -2105,11 +2217,12 @@ theorem Iter.fold_filterWithPostcondition {α β δ : Type w}
     Triple P ((it.filterWithPostcondition f).fold (init := init) g) Q eQ := by
   rwa [Std.Iter.fold_filterWithPostcondition]
 
-theorem Iter.fold_filterM {α β δ : Type w}
+@[lspec]
+theorem Spec.Iter.fold_filterM {α β δ : Type w}
     {n : Type w → Type w'}
     {l : Type w} {e : Type w}
     [Iterator α Id β] [Finite α Id]
-    [Monad n] [MonadAttach n] [LawfulMonad n] [WeaklyLawfulMonadAttach n] [WPMonad n l e]
+    [Monad n] [MonadAttach n] [LawfulMonad n] [WeaklyLawfulMonadAttach n] [AssertionLang l] [ExceptAssertionLang e] [WPMonad n l e]
     [IteratorLoop α Id n] [LawfulIteratorLoop α Id n]
     {f : β → n (ULift Bool)} {g : δ → β → δ} {init : δ} {it : Iter (α := α) β}
     {P : l} {Q : δ → l} {eQ : e}
@@ -2120,6 +2233,7 @@ theorem Iter.fold_filterM {α β δ : Type w}
 end Iterators
 
 
+@[lspec]
 theorem Spec.forIn'_array {xs : Array α} {init : β} {f : (a : α) → a ∈ xs → β → m (ForInStep β)}
     (inv : Invariant xs.toList β l)
     (eInv : e)
@@ -2138,6 +2252,7 @@ theorem Spec.forIn'_array {xs : Array α} {init : β} {f : (a : α) → a ∈ xs
       eInv := by
   cases xs; simp; apply Spec.forIn'_list inv eInv step
 
+@[lspec]
 theorem Spec.forIn_array {xs : Array α} {init : β} {f : α → β → m (ForInStep β)}
     (inv : Invariant xs.toList β l)
     (eInv : e)
@@ -2156,6 +2271,7 @@ theorem Spec.forIn_array {xs : Array α} {init : β} {f : α → β → m (ForIn
       eInv := by
   cases xs; simp; apply Spec.forIn_list inv eInv step
 
+@[lspec]
 theorem Spec.foldlM_array [LawfulMonad m]
     {xs : Array α} {init : β} {f : β → α → m β}
     (inv : Invariant xs.toList β l)
@@ -2172,93 +2288,5 @@ theorem Spec.foldlM_array [LawfulMonad m]
       (fun b => inv (⟨xs.toList, [], by simp⟩, b))
       eInv := by
   cases xs; simp; apply Spec.foldlM_list inv eInv step
-
-/--
-The type of loop invariants used by the specifications of `for ... in ...` loops over strings.
-A loop invariant is a function mapping the current position and state to a lattice element.
--/
-abbrev StringInvariant (s : String) (β : Type u)
-    (l : Type u) :=
-  (s.Pos × β → l)
-
-theorem Spec.forIn_string
-    {s : String} {init : β} {f : Char → β → m (ForInStep β)}
-    (inv : StringInvariant s β l)
-    (eInv : e)
-    (step : ∀ pos b (h : pos ≠ s.endPos),
-      Triple
-        (inv (pos, b))
-        (f (pos.get h) b)
-        (fun r => match r with
-          | .yield b' => inv (pos.next h, b')
-          | .done b' => inv (s.endPos, b'))
-        eInv) :
-    Triple (inv (s.startPos, init)) (forIn s init f) (fun b => inv (s.endPos, b)) eInv := by
-  suffices h : ∀ (p : s.Pos) (t₁ t₂ : String) (h : p.Splits t₁ t₂),
-      Triple (inv (p, init)) (forIn t₂.toList init f) (fun b => inv (s.endPos, b)) eInv by
-    simpa using h s.startPos _ _ s.splits_startPos
-  intro p
-  induction p using String.Pos.next_induction generalizing init with
-  | next p hp ih =>
-    intro t₁ t₂ hsp
-    obtain ⟨t₂, rfl⟩ := hsp.exists_eq_singleton_append hp
-    simp only [String.toList_append, String.toList_singleton, List.cons_append, List.nil_append,
-      List.forIn_cons]
-    apply Triple.bind
-    case hx => exact step _ _ hp
-    case hf =>
-      intro r
-      cases r with
-      | yield b => exact ih _ _ hsp.next
-      | done b => exact Triple.pure _ (by dsimp; exact Lean.Order.PartialOrder.rel_refl)
-  | endPos =>
-    intro t₁ t₂ hsp
-    obtain ⟨-, rfl⟩ := String.splits_endPos_iff.mp hsp
-    simp only [String.toList_empty, List.forIn_nil]
-    exact Triple.pure init Lean.Order.PartialOrder.rel_refl
-
-/--
-The type of loop invariants used by the specifications of `for ... in ...` loops over string slices.
-A loop invariant is a function mapping the current position and state to a lattice element.
--/
-abbrev StringSliceInvariant (s : String.Slice) (β : Type u)
-    (l : Type u) :=
-  (s.Pos × β → l)
-
-theorem Spec.forIn_stringSlice
-    {s : String.Slice} {init : β} {f : Char → β → m (ForInStep β)}
-    (inv : StringSliceInvariant s β l)
-    (eInv : e)
-    (step : ∀ pos b (h : pos ≠ s.endPos),
-      Triple
-        (inv (pos, b))
-        (f (pos.get h) b)
-        (fun r => match r with
-          | .yield b' => inv (pos.next h, b')
-          | .done b' => inv (s.endPos, b'))
-        eInv) :
-    Triple (inv (s.startPos, init)) (forIn s init f) (fun b => inv (s.endPos, b)) eInv := by
-  suffices h : ∀ (p : s.Pos) (t₁ t₂ : String) (h : p.Splits t₁ t₂),
-      Triple (inv (p, init)) (forIn t₂.toList init f) (fun b => inv (s.endPos, b)) eInv by
-    simpa using h s.startPos _ _ s.splits_startPos
-  intro p
-  induction p using String.Slice.Pos.next_induction generalizing init with
-  | next p hp ih =>
-    intro t₁ t₂ hsp
-    obtain ⟨t₂, rfl⟩ := hsp.exists_eq_singleton_append hp
-    simp only [String.toList_append, String.toList_singleton, List.cons_append, List.nil_append,
-      List.forIn_cons]
-    apply Triple.bind
-    case hx => exact step _ _ hp
-    case hf =>
-      intro r
-      cases r with
-      | yield b => exact ih _ _ hsp.next
-      | done b => exact Triple.pure _ (by dsimp; exact Lean.Order.PartialOrder.rel_refl)
-  | endPos =>
-    intro t₁ t₂ hsp
-    obtain ⟨-, rfl⟩ := String.Slice.splits_endPos_iff.mp hsp
-    simp only [String.toList_empty, List.forIn_nil]
-    exact Triple.pure init Lean.Order.PartialOrder.rel_refl
 
 end Std.Do'
